Work on binomial heap functional correctness
I ended up developing a bunch of background theory. I'm not sure how
much of it was necessary.

src/BinomialHeap.v
@@ -1,15 +1,15 @@
 (* Overview
 
-- Pure implementation of binomial heaps: [Tree], [Heap], [link], [rank], 
+-- Pure implementation of binomial heaps: [Tree], [Heap], [link], [rank],
     [root], [insTree], [insert], [merge], [removeMinTree], [findMin], [deleteMin]
-- Clairvoyant-monadic implementation: [TreeA], [HeapA], [linkA], [rankA], 
+-- Clairvoyant-monadic implementation: [TreeA], [HeapA], [linkA], [rankA],
     [rootA], [insTreeA], [insertA], [mergeA], [removeMinTreeA], [findMinA], [deleteMinA]
 
 NEW
-- Demand functions: 
+- Demand functions:
 - (Physicist's method) Debt/negative potential: [debt]
 - Amortized cost specifications:
-- "API traces" with sharing: 
+- "API traces" with sharing:
 - Final theorem (statement and proof):
     the cost of executing a trace with [n] operations is ?
 
@@ -24,78 +24,334 @@ From Clairvoyance Require Import Core Approx ApproxM List ListA Misc Tick Demand
 Import Tick.Notations.
 #[local] Open Scope tick_scope.
 
+Set Implicit Arguments.
+
+(* I have had some problems with inversion_clear. This does the same thing, but
+   hopefully better. *)
+Tactic Notation "invert_clear" hyp(H) "as" simple_intropattern(pat) :=
+  let HI := fresh "HI" in
+  pose I as HI;
+  inversion H as pat;
+  repeat lazymatch goal with
+    | _ : ?x = ?y |- _ => subst x + subst y
+    end;
+  clear HI;
+  clear H.
+
+Tactic Notation "invert_clear" hyp(H) :=
+  invert_clear H as [ ].
+
+Tactic Notation "invert_clear" integer(n) "as" simple_intropattern(pat) :=
+  progress (intros until n);
+  match goal with
+  | H : _ |- _ => invert_clear H as pat
+  end.
+
+(* For some reason, trying to chain this into the above notation causes
+   problems. *)
+Tactic Notation "invert_clear" integer(n) :=
+  progress (intros until n);
+  match goal with
+  | H : _ |- _ => invert_clear H as [ ]
+  end.
+
+(* Tactic to invert/subst/clear a single hypothesis of the form
+
+   P x1 x2 ... (C y1 y2 ... yn) ... xn
+
+   where C is a constructor. This is a common way to make progress. *)
+Ltac invert_constructor :=
+  let rec head_is_constructor t := match t with
+                                   | ?f ?x => head_is_constructor f
+                                   | _ => is_constructor t
+                                   end in
+  let rec should_invert T := match T with
+                             | ?P ?x => head_is_constructor x + should_invert P
+                             end in
+  intros;
+  match goal with
+  | H : ?T |- _ => should_invert T; invert_clear H
+  end.
+
+Inductive LiftT A (P : A -> Prop) : T A -> Prop :=
+| LiftT_Undefined : LiftT P Undefined
+| LiftT_Thunk x : P x -> LiftT P (Thunk x).
+#[global] Hint Constructors LiftT : core.
+
+Lemma LiftT_impl A (P Q : A -> Prop) :
+  (forall x, P x -> Q x) -> forall x, LiftT P x -> LiftT Q x.
+Proof.
+  intros until x. destruct 1; auto.
+Qed.
+#[global] Hint Resolve LiftT_impl : core.
+
+(* Lift a binary relation to T in a way that preserves the less-defined
+   relation. *)
+Inductive LiftT2 A B (R : A -> B -> Prop) : T A -> T B -> Prop :=
+| LiftT2_Undefined yD : LiftT2 R Undefined yD
+| LiftT2_Thunk x y : R x y -> LiftT2 R (Thunk x) (Thunk y).
+#[global] Hint Constructors LiftT2 : core.
+
+Lemma LiftT2_impl A B (R1 R2 : A -> B -> Prop) :
+  (forall x y, R1 x y -> R2 x y) -> forall xD yD, LiftT2 R1 xD yD -> LiftT2 R2 xD yD.
+Proof.
+  intros until yD. destruct 1; auto.
+Qed.
+#[global] Hint Resolve LiftT2_impl : core.
+
+Lemma LiftT2_refl A (R : A -> A -> Prop) :
+  (forall x, R x x) -> forall xD, LiftT2 R xD xD.
+Proof.
+  destruct xD; auto.
+Qed.
+#[global] Hint Resolve LiftT2_refl : core.
+
+Lemma LiftT2_trans A (R : A -> A -> Prop) :
+  (forall x y z, R x y -> R y z -> R x z) ->
+  forall xD yD zD, LiftT2 R xD yD -> LiftT2 R yD zD -> LiftT2 R xD zD.
+Proof.
+  inversion 2; inversion 1; eauto.
+Qed.
+#[global] Hint Resolve LiftT2_trans : core.
+
+Lemma LiftT_diag_LiftT2 A (R : A -> A -> Prop) xD :
+  LiftT (fun x => R x x) xD <-> LiftT2 R xD xD.
+Proof.
+  split; invert_clear 1; auto.
+Qed.
+#[global] Hint Resolve -> LiftT_diag_LiftT2 : core.
+#[global] Hint Resolve <- LiftT_diag_LiftT2 : core.
+
+Lemma LiftT2_less_defined A `{LessDefined A} (R : A -> A -> Prop) (x y : T A) :
+  LiftT2 less_defined x y <-> x `less_defined` y.
+Proof.
+  split; invert_clear 1; auto.
+Qed.
+#[global] Hint Resolve -> LiftT2_less_defined : core.
+#[global] Hint Resolve <- LiftT2_less_defined : core.
+
+Ltac invert_LiftT :=
+  match goal with
+  | H : LiftT _ _ |- _ => invert_clear H
+  | H : LiftT2 _ _ _ |- _ => invert_clear H
+  end.
+
+Inductive ForallA A (P : A -> Prop) : listA A -> Prop :=
+| ForallA_NilA : ForallA P NilA
+| ForallA_ConsA x xs : LiftT P x -> LiftT (ForallA P) xs -> ForallA P (ConsA x xs).
+#[global] Hint Constructors ForallA : core.
+
+Lemma ForallA_impl A (P Q : A -> Prop) :
+  (forall x, P x -> Q x) -> forall xs, ForallA P xs -> ForallA Q xs.
+Proof.
+  induction xs; repeat invert_constructor; eauto.
+Qed.
+#[global] Hint Resolve ForallA_impl : core.
+
+(* Lift a binary relation to listA in a way that preserves the less-defined
+   relation. *)
+Inductive ForallA2 A B (R : A -> B -> Prop) : listA A -> listA B -> Prop :=
+| ForallA2_NilA : ForallA2 R NilA NilA
+| ForallA2_ConsA x y xs ys : LiftT2 R x y -> LiftT2 (ForallA2 R) xs ys -> ForallA2 R (ConsA x xs) (ConsA y ys).
+#[global] Hint Constructors ForallA2 : core.
+
+Lemma ForallA2_impl A B (R1 R2 : A -> B -> Prop) :
+  (forall x y, R1 x y -> R2 x y) -> forall xs ys, ForallA2 R1 xs ys -> ForallA2 R2 xs ys.
+Proof.
+  induction xs; repeat invert_constructor; eauto.
+Qed.
+#[global] Hint Resolve ForallA2_impl : core.
+
+Lemma ForallA2_refl A (R : A -> A -> Prop) :
+  (forall x, R x x) -> forall xs, ForallA2 R xs xs.
+Proof.
+  induction xs; auto.
+Qed.
+#[global] Hint Resolve ForallA2_refl : core.
+
+Lemma ForallA2_trans A (R : A -> A -> Prop) :
+  (forall x y z, R x y -> R y z -> R x z) ->
+  forall xs ys zs, ForallA2 R xs ys -> ForallA2 R ys zs -> ForallA2 R xs zs.
+Proof.
+  intros ? xs ys zs Hxsys Hyszs. revert xs zs Hxsys Hyszs.
+  induction ys; repeat invert_constructor; eauto.
+Qed.
+#[global] Hint Resolve ForallA2_trans : core.
+
+Lemma ForallA_diag_ForallA2 A (R : A -> A -> Prop) xs :
+  ForallA (fun x => R x x) xs <-> ForallA2 R xs xs.
+Proof.
+  split; induction xs; repeat invert_constructor; auto.
+Qed.
+#[global] Hint Resolve -> ForallA_diag_ForallA2 : core.
+#[global] Hint Resolve <- ForallA_diag_ForallA2 : core.
+
+Lemma ForallA2_less_defined A `{LessDefined A} (xs ys : listA A) : ForallA2 less_defined xs ys <-> xs `less_defined` ys.
+Proof.
+  split.
+  - revert ys. induction xs; repeat invert_constructor; auto.
+  - induction 1; auto.
+Qed.
+#[global] Hint Resolve -> ForallA2_less_defined : core.
+#[global] Hint Resolve <- ForallA2_less_defined : core.
+
 Notation A := nat (only parsing).
 
+Unset Elimination Schemes.
+
 Inductive Tree : Type :=
-  | Node : nat -> A -> list Tree -> Tree.
+| Node : forall (n : nat) (x : A) (ts : list Tree), Tree.
+
+Lemma Tree_ind (P : Tree -> Prop) :
+    (forall (n : nat) (x : A) (ts : list Tree), Forall P ts -> P (Node n x ts)) ->
+    forall (t : Tree), P t.
+Proof.
+  intros H. fix SELF 1.
+  destruct t. apply H. induction ts; auto.
+Qed.
 
 Inductive TreeA : Type :=
-  | NodeA : T nat -> T A -> T (listA TreeA) -> TreeA.
+| NodeA : forall (nD : T nat) (xD : T A) (tsD : T (listA TreeA)), TreeA.
 
-Canonical AA_Tree :=
-  {| carrier := Tree
-  ;  approx := TreeA
-  ;  AA_Setoid := TODO
-  ;  AA_IsAA := TODO
-  ;  AA_IsAS := TODO
-  |}.
+Lemma TreeA_ind : forall (P : TreeA -> Prop),
+    (forall (nD : T nat) (xD : T A) (tsD : T (listA TreeA)), LiftT (ForallA P) tsD -> P (NodeA nD xD tsD)) ->
+    forall (tD : TreeA), P tD.
+Proof.
+  intros ? H. fix SELF 1.
+  destruct tD. apply H. destruct tsD as [ ts | ].
+  1: induction ts as [ | tD | tD ]. 2, 3: destruct tD.
+  all: repeat constructor; try invert_constructor; auto.
+Qed.
 
-Record Heap : Type := MkHeap
-  { trees : list Tree }.
+Inductive LessDefined_TreeA : LessDefined TreeA :=
+| less_defined_TreeA_NodeA n1D n2D x1D x2D ts1D ts2D :
+  n1D `less_defined` n2D ->
+  x1D `less_defined` x2D ->
+  (* Need to pass instance explicitly, because LessDefined_TreeA is not yet
+     registered. *)
+  @less_defined _ (@LessDefined_T _ (@LessDefined_list _ LessDefined_TreeA)) ts1D ts2D ->
+  LessDefined_TreeA (NodeA n1D x1D ts1D) (NodeA n2D x2D ts2D).
+#[global] Existing Instance LessDefined_TreeA.
+#[global] Hint Constructors LessDefined_T : core.
 
-Record HeapA : Type := MkHeapA
-  { treesA : T (listA TreeA) }.
+Lemma LessDefined_TreeA_ind :
+  forall (P : TreeA -> TreeA -> Prop),
+    (forall (n1D n2D : T nat) (x1D x2D : T nat) (ts1D ts2D : T (listA TreeA)),
+        n1D `less_defined` n2D ->
+        x1D `less_defined` x2D ->
+        LiftT2 (ForallA2 P) ts1D ts2D ->
+        P (NodeA n1D x1D ts1D) (NodeA n2D x2D ts2D)) ->
+    forall (t1 t2 : TreeA), LessDefined_TreeA t1 t2 -> P t1 t2.
+Proof.
+  intros P H. fix SELF 3.
+  intros t1 t2 Hts. destruct Hts as [ n1D n2D x1D x2D ts1D ts2D HnD HxD HtsD ].
+  apply H. 1, 2: assumption.
+  invert_clear HtsD as [ | ts1 ts2 Hts12 ]; constructor.
+  induction Hts12 as [ | t1D t2D ? HtD12 | t1D t2D ? ? HtD12 ].
+  1: auto.
+  1, 2: invert_clear HtD12; auto.
+Qed.
 
-Canonical AA_Heap : AA :=
-  {| carrier := Heap
-  ;  approx := T HeapA
-  ;  AA_Setoid := TODO
-  ;  AA_IsAA := TODO
-  ;  AA_IsAS := TODO
-  |}.
+Set Elimination Schemes.
+
+#[global] Instance LessDefined_TreeA_reflexive : Reflexive LessDefined_TreeA.
+Proof.
+  pose (Reflexive_LessDefined_T (a := nat)).
+  unfold Reflexive. intro t. induction t. constructor.
+  3: invert_LiftT.
+  all: auto.
+Qed.
+
+#[global] Instance LessDefined_TreeA_transitive : Transitive LessDefined_TreeA.
+Proof.
+  pose (Transitive_LessDefined_T (a := nat)).
+  unfold Transitive. intros t1 t2 t3 Ht12 Ht23.
+  revert t2 t3 Ht12 Ht23. induction t1 as [ n1D x1D ts1D HtsD1 ]. intros.
+  invert_clear Ht12 as [ ? n2D ? x2D ? ts2D HnD12 HxD12 HtsD12 ].
+  invert_clear Ht23 as [ ? nD3 ? xD3 ? ts3D HnD23 HxD23 HtsD23 ].
+  constructor. 1, 2: eauto.
+  invert_clear HtsD1 as [ | ts1 ]. 1: auto.
+  invert_clear HtsD12 as [ | ? ts2 Hts12 ].
+  invert_clear HtsD23 as [ | ? ts3 Hts23 ].
+  constructor.
+  revert ts2 ts3 Hts12 Hts23. induction ts1;
+    repeat (invert_constructor + invert_LiftT); repeat constructor;
+    try (match goal with | H : _ |- _ => eapply H end);
+    eauto.
+Qed.
+
+Add Relation TreeA LessDefined_TreeA
+    reflexivity proved by LessDefined_TreeA_reflexive
+    transitivity proved by LessDefined_TreeA_transitive
+    as LessDefined_TreeA_Relation.
+
+(** Exact_list depends on an Exact instance for the element type, but the
+    element type here is Tree. We can't hand out Exact_Tree while it's being
+    constructed, because that won't pass the termination checker. So we have to
+    roll our own Exact_list here. *)
+#[global] Instance Exact_Tree : Exact Tree TreeA := fix Exact_Tree t :=
+  let fix Exact_trees (ts : list Tree) : listA TreeA :=
+    match ts with
+    | [] => NilA
+    | t :: ts' => ConsA (Thunk (Exact_Tree t)) (Thunk (Exact_trees ts'))
+    end
+  in match t with
+     | Node n x ts => NodeA (exact n) (exact x) (Thunk (Exact_trees ts))
+     end.
+
+(** However, once we have defined Exact_Tree, we can show that it behaves the
+    same as if it had been defined using Exact_list. (Of course, this depends
+    recursively on the definition of Exact_Tree. There's no way around that.) *)
+Lemma Exact_Tree_Exact_list (t : Tree) :
+  exact t = match t with
+            | Node n x ts => NodeA (exact n) (exact x) (exact ts)
+            end.
+Proof.
+  induction t as [ ? ? ? IH ]. induction IH as [ | ? ? ? ? IHIH ].
+  - reflexivity.
+  - cbv. simp exact_listA. repeat f_equal.
+    cbv in IHIH. injection IHIH. trivial.
+Qed.
+#[global] Hint Resolve Exact_Tree_Exact_list : core.
 
 Definition link (t1 t2 : Tree) : Tree :=
   match t1, t2 with
   | Node r1 v1 c1, Node r2 v2 c2 => if leb v1 v2
-    then Node (r1 + 1) v1 (t2 :: c1)
-    else Node (r2 + 1) v2 (t1 :: c2)
-  end.
-
-(* Encoding of Node *)
-(* Currently unused, just pattern-match on it instead *)
-Definition NodeD (t : TreeA) : Tick (T nat * T A * T (listA TreeA)) :=
-  Tick.ret
-  match t with
-  | NodeA n x ts => (n, x, ts)
-  end.
-
-Definition TNodeD (t : T TreeA) : Tick (T nat * T A * T (listA TreeA)) :=
-  Tick.ret
-  match t with
-  | Thunk (NodeA n x ts) => (n, x, ts)
-  | Undefined => (Undefined, Undefined, Undefined)
+                                    then Node (r1 + 1) v1 (t2 :: c1)
+                                    else Node (r2 + 1) v2 (t1 :: c2)
   end.
 
 Definition linkD (t1 t2 : Tree) (d : TreeA) : Tick (T TreeA * T TreeA) :=
   match t1, t2 with
   | Node r1 v1 c1, Node r2 v2 c2 =>
-    if leb v1 v2 then
-      match d with
-      | NodeA rD v1D tsD =>
-        let '(t2D, c1D) := TConsD tsD in
-        Tick.ret (Thunk (NodeA (exact r1) v1D c1D), t2D)
-      end
-    else
-      match d with
-      | NodeA rD v2D tsD =>
-        let '(t1D, c2D) := TConsD tsD in
-        Tick.ret (t1D, Thunk (NodeA (exact r2) v2D c2D))
-      end
+      if leb v1 v2 then
+        match d with
+        | NodeA rD v1D tsD =>
+            let '(t2D, c1D) := TConsD tsD in
+            Tick.ret (Thunk (NodeA (exact r1) v1D c1D), t2D)
+        end
+      else
+        match d with
+        | NodeA rD v2D tsD =>
+            let '(t1D, c2D) := TConsD tsD in
+            Tick.ret (t1D, Thunk (NodeA (exact r2) v2D c2D))
+        end
   end.
 
-(* Currently unused, just pattern-match *)
-Definition MkHeapD (d : HeapA) : Tick (T (listA TreeA)) :=
-  Tick.ret (treesA d).
+Lemma link_approx (t1 t2 : Tree) (outD : TreeA)
+  : outD `is_approx` link t1 t2 ->
+    Tick.val (linkD t1 t2 outD) `is_approx` (t1, t2).
+Proof.
+  destruct t1 as [ n1 x1 ts1 ], t2 as [ n2 x2 ts2 ]. simpl.
+  destruct (x1 <=? x2); cbn; repeat invert_constructor; repeat constructor; auto.
+Qed.
+#[global] Hint Resolve link_approx : core.
+
+Definition ConsD {A} (xs : listA A) : T A * T (listA A) :=
+  match xs with
+  | ConsA x ys => (x, ys)
+  | _ => (Undefined, Undefined) (* should not happen *)
+  end.
 
 Definition rank (t : Tree) : nat :=
   match t with
@@ -112,11 +368,77 @@ Fixpoint insTree (t : Tree) (ts : list Tree) : list Tree :=
   match ts with
   | [] => [t]
   | t' :: ts' => if rank t <? rank t'
-    then t :: ts
-    else insTree (link t t') ts' (*t and t' should have the same rank*)
+                 then t :: ts
+                 else insTree (link t t') ts' (*t and t' should have the same rank*)
   end.
 
+Lemma insTree_is_cons (t : Tree) (ts : list Tree) : exists t' ts', insTree t ts = t' :: ts'.
+Proof.
+  revert t. induction ts; intro; simpl.
+  2: destruct (rank t <? rank a).
+  all: eauto.
+Qed.
+#[global] Hint Resolve insTree_is_cons : core.
+
+#[global] Instance Lub_TreeA : Lub TreeA :=
+  fix Lub_TreeA t1 t2 :=
+    let fix lub_list_TreeA (ts1 ts2 : listA TreeA) :=
+      match ts1, ts2 with
+      | NilA, NilA => NilA
+      | ConsA t1 ts1, ConsA t2 ts2 => ConsA (lub_T Lub_TreeA t1 t2) (lub_T lub_list_TreeA ts1 ts2)
+      | _, _ => NilA
+      end in
+    match t1, t2 with
+    | NodeA n1 x1 ts1, NodeA n2 x2 ts2 => NodeA (lub n1 n2) (lub x1 x2) (lub_T lub_list_TreeA ts1 ts2)
+    end.
+
+(* Lemma Lub_TreeA_Lub_listA (t1 t2 : TreeA) : *)
+(*   lub t1 t2 = match t1, t2 with *)
+(*               | NodeA n1 x1 ts1, NodeA n2 x2 ts2 => NodeA (lub n1 n2) (lub x1 x2) (lub ts1 ts2) *)
+(*               end. *)
+(* Proof. *)
+(*   induction t1, t2. destruct H. 1: auto. destruct t1. 2: auto. *)
+(*   enough (lub x0 x1 = match x0, x1 with *)
+(*                       | NilA, NilA => NilA *)
+(*                       | ConsA t1 ts1, ConsA t2 ts2 => ConsA (lub_T Lub_TreeA t1 t2) (lub_T lub_list_TreeA ts1 ts2) *)
+(*                       | _, _ => NilA *)
+(*                       end). *)
+(*   unfold lub, Lub_TreeA in *. simpl. f_equal. f_equal. *)
+(*   apply ForallA_impl in H with (Q := fun t1 => *)
+
+(*   unfold lub, Lub_TreeA, lub in *. f_equal. *)
+(*   cbn in *. destruct t1. 2: auto. *)
+(*   f_equal. unfold lub, List.Lub_listA, List.lub_listA in *. *)
+(*   apply Forall_impl with (Q := *)
+
+(*   unfold lub_T, Lub_T, lub, List.Lub_listA, List.lub_listA. *)
+(*   apply Forall_impl with (Q := fun ts2 => lub_T *)
+(*   unfold lub. destruct t1. simpl. *)
+
+(*   - induction H; auto. *)
+(*     + induction H0. cbn. destruct t1. induction x1. *)
+(*       * auto. *)
+(*       * unfold lub, lub_T. destruct x0, x1; auto. *)
+(*   - induction H0. *)
+
+(*   destruct t1 as [n1 x1 ts1], t2 as [n2 x2 ts2]. unfold lub, Lub_TreeA. f_equal. *)
+(*   clear n1. clear x1. clear n2. clear x2. *)
+(*   unfold Lub_T, lub_T. destruct ts1 as [ts1 |], ts2 as [ts2 |]; auto. f_equal. *)
+(*   induction ts1, ts2; auto. *)
+(*   - unfold lub. simpl. f_equal. *)
+(*   (* - unfold lub, List.Lub_listA, List.lub_listA, lub_T. f_equal. destruct x0, x3; try (destruct x, x0); auto. f_equal. f_equal. unfold Lub_T. destruct t, t2; auto. *) *)
+(*   (*   destruct x, x0; auto. f_equal. unfold Lub_T. destruct t, t2; auto *) *)
+(*   (* - unfold lub, List.Lub_listA, List.lub_listA. f_equal. *) *)
+(*   (* induction ts1 as [| t1 ts1 | t1 ts1 IHts1], ts2 as [| t2 ts2 IHts2]; auto. *) *)
+(*   (* - unfold lub. unfold Lub_T. f_equal. unfold lub. destruct t1, t2; auto. *) *)
+(*   (* - destruct ts2; auto. *) *)
+(*   (* - *) *)
+
+(*     (* - *) *)
+(* Admitted. *)
+
 Definition strictD (t : Tree) (x' : T TreeA) : T TreeA := lub x' (Thunk (NodeA (exact (rank t)) Undefined Undefined)).
+
 Definition strictConsD {A} (xs' : T (listA A)) : T (listA A) := lub xs' (Thunk (ConsA Undefined Undefined)).
 
 (* [d] is an approximation of the output [insTree t ts] *)
@@ -126,1009 +448,1164 @@ Fixpoint insTreeD (t : Tree) (ts : list Tree) (d : listA TreeA) : Tick (T TreeA 
     (* [d] is an approximation of [t :: nil] *)
     (* ConsD inverts it and returns approximations of [t] and [nil] (which is ignored) *)
     let '(tD, _) := ConsD d in
-    (* To find out what to return, we enumerate all of the uses of the arguments of [insTree]:
-       - [t] was only used in the output list, corresponding to the demand [tD]
-       - [ts] was used in [match], so its demand must at least be [Thunk NilA], which is fully defined.
-    *)
+    (* To find out what to return, we enumerate all of the uses of the arguments of [insTree]: *)
+(*        - [t] was only used in the output list, corresponding to the demand [tD] *)
+(*        - [ts] was used in [match], so its demand must at least be [Thunk NilA], which is fully defined. *)
+(*     *)
     Tick.ret (tD, Thunk NilA)
   | t' :: ts' => if rank t <? rank t'
     then (* [d] is an approximation of [t :: ts] *)
          let '(tD, tsD) := ConsD d in
-         (* [t] occurs in the result [t :: ts] (with demand [tD]), and also to compare its rank,
-            so we use [strictD] to give its demand a defined rank.
-            [ts] was also pattern-matched on, so we similarly require an annotation
-            to make its demand not [Undefined]. *)
+         (* [t] occurs in the result [t :: ts] (with demand [tD]), and also to compare its rank, *)
+(*             so we use [strictD] to give its demand a defined rank. *)
+(*             [ts] was also pattern-matched on, so we similarly require an annotation *)
+(*             to make its demand not [Undefined]. *)
          Tick.ret (strictD t tD, strictConsD tsD)
-    else (* The result of [insTree] is a recursive call. So we recursively compute the
-            demand on its arguments: [lD] is the demand on [link t t'], and [ts'D] is the demand
-            on [ts]. *)
+    else (* The result of [insTree] is a recursive call. So we recursively compute the *)
+(*             demand on its arguments: [lD] is the demand on [link t t'], and [ts'D] is the demand *)
+(*             on [ts]. *)
          let+ (lD, ts'D) := insTreeD (link t t') ts' d in
-         (* [linkD] takes [lD] to compute a demand on [t] and [t'].
+         (* [linkD] takes [lD] to compute a demand on [t] and [t']. *)
 
-            Demand functions return results wrapped in [T] (so that [Undefined]
-            may indicate an unused argument), but the input demand is not wrapped in [T]
-            (since there is no point in calling this if the argument is unused).
-            We use [thunkD] to apply a demand function on a demand wrapped in
-            [T] (here [lD]), usually coming from a pattern or another function. *)
+(*             Demand functions return results wrapped in [T] (so that [Undefined] *)
+(*             may indicate an unused argument), but the input demand is not wrapped in [T] *)
+(*             (since there is no point in calling this if the argument is unused). *)
+(*             We use [thunkD] to apply a demand function on a demand wrapped in *)
+(*             [T] (here [lD]), usually coming from a pattern or another function. *)
          let+ (tD, t'D) := thunkD (linkD t t') lD in
          Tick.ret (strictD t tD, Thunk (ConsA t'D ts'D))
   end.
 
-Definition insert (x : A) (hp : Heap)
-  : Heap :=
-  MkHeap (insTree (Node 0 x []) (trees hp)).
+Lemma insTree_approx (t : Tree) (ts : list Tree) (outD : listA TreeA)
+  : outD `is_approx` insTree t ts ->
+    Tick.val (insTreeD t ts outD) `is_approx` (t, ts).
+Proof.
+  (* induction ts, outD;  unfold less_defined; simpl; try (destruct (rank t <? rank a)). constructor. auto. simpl. invert_constructors; repeat constructor; auto. *)
+  (* - unfold strictD. simpl. *)
+  (* - *)
+  (* unfold exact, Exact_T. *)
 
-Definition insertD (x : A) (hp : Heap) (d : HeapA) : Tick (T A * T HeapA) :=
-  let+ (tD, trees_hpD) := thunkD (insTreeD (Node 0 x []) (trees hp)) (treesA d) in
-  let+ (_, xD, _) := TNodeD tD in
-  Tick.ret (xD, Thunk (MkHeapA trees_hpD)).
-
-
-Fixpoint mergeAux (trs1 trs2 : list Tree) : list Tree :=
-  match trs1 with
-  | [] => trs2
-  | t1 :: trs1' => let fix merge_trs1 trsR :=
-    match trsR with
-    | [] => trs1
-    | t2 :: trs2' =>
-      match Nat.compare (rank t1) (rank t2) with
-      | Lt => t1 :: (mergeAux trs1' trsR)
-      | Eq => insTree (link t1 t2) (mergeAux trs1' trs2')
-      | Gt => t2 :: merge_trs1 trs2'
-      end
-    end in
-    merge_trs1 trs2
-  end.
-
-Definition merge (hp1 hp2 : Heap) : Heap :=
-  MkHeap (mergeAux (trees hp1) (trees hp2)).
-
-Fixpoint mergeAuxD (trs1 trs2 : list Tree) (d : listA TreeA) : Tick (T (listA TreeA) * T (listA TreeA)) :=
-  match trs1 with
-  | [] => Tick.ret (Thunk NilA, Thunk d)
-  | t1 :: trs1' => let fix merge_trs1 trsR (dR : listA TreeA) : Tick (T (listA TreeA) * T (listA TreeA)) :=
-    (* here we compute the demand on [trs1] and [trsR] *)
-    match trsR with
-    | [] => Tick.ret (Thunk dR, Thunk NilA)
-    | t2 :: trs2' =>
-      match Nat.compare (rank t1) (rank t2) with
-      | Lt =>
-        let '(t1D, mD) := ConsD dR in
-        let+ (trs1'D, trsRD) := thunkD (mergeAuxD trs1' trsR) mD in
-        Tick.ret (Thunk (ConsA (strictD t1 t1D) trs1'D), strictConsD trsRD)
-      | Eq =>
-        let+ (lD, mD) := insTreeD (link t1 t2) (mergeAux trs1' trs2') dR in
-        let+ (t1D, t2D) := thunkD (linkD t1 t2) lD in
-        let+ (trs1'D, trs2'D) := thunkD (mergeAuxD trs1' trs2') mD in
-        Tick.ret (Thunk (ConsA (strictD t1 t1D) trs1'D), Thunk (ConsA (strictD t2 t2D) trs2'D))
-      | Gt =>
-        let '(t2D, mD) := ConsD dR in
-        let+ (trs1D, trs2'D) := thunkD (merge_trs1 trs2') mD in
-        Tick.ret (trs1D, Thunk (ConsA (strictD t2 t2D) trs2'D))
-      end
-    end in
-    let+ (trs1D, trs2D) := merge_trs1 trs2 d in
-    Tick.ret (strictConsD trs1D, trs2D)
-  end.
-
-Definition mergeD (hp1 hp2 : Heap) (d : HeapA) : Tick (T HeapA * T HeapA) :=
-  let+ (ts1D, ts2D) := thunkD (mergeAuxD (trees hp1) (trees hp2)) (treesA d) in
-  Tick.ret (Thunk (MkHeapA ts1D), Thunk (MkHeapA ts2D)).
-
-Fixpoint removeMinAux (ts : list Tree) : option (Tree * list Tree) :=
-  match ts with
-  | [] => None
-  | t :: ts' => match removeMinAux ts' with
-    | None => Some (t, [])
-    | Some (t', ts'') => if leb (root t) (root t')
-      then Some (t, ts')
-      else Some (t', t :: ts'')
-    end
-  end.
-
-Definition SomeD {A} `{Bottom A} (x : option A) : A :=
-  match x with
-  | Some y => y
-  | _ => bottom
-  end.
-
-Fixpoint removeMinAuxD (ts : list Tree) (d : option (T TreeA * T (listA TreeA)))
-  : Tick (T (listA TreeA)) :=
-  match ts with
-  | [] => Tick.ret (Thunk NilA)
-  | t :: ts' => match removeMinAux ts' with
-    | None =>
-      let (tD, _) := SomeD d in
-      let+ ts'D := removeMinAuxD ts' None in
-      Tick.ret (Thunk (ConsA tD ts'D))
-    | Some (t', ts'') => if leb (root t) (root t')
-      then
-        let '(tD, ts'D) := SomeD d in
-        let+ ts'D := removeMinAuxD ts' (Some (strictD t' Undefined, Undefined)) in
-        Tick.ret (Thunk (ConsA tD ts'D))
-      else
-        let '(t'D, tts''D) := SomeD d in
-        let '(tD, ts''D) := TConsD tts''D in
-        let+ ts'D := removeMinAuxD ts' (Some (strictD t' t'D, ts''D)) in
-        Tick.ret (Thunk (ConsA tD ts'D))
-    end
-  end.
-
-Definition removeMinTree (hp : Heap)
-  : option ((Tree) * (Heap)) :=
-  match removeMinAux (trees hp) with
-  | Some (t, ts) => Some (t, MkHeap ts)
-  | None => None
-  end.
-
-Definition removeMinTreeD (hp : Heap) (d : option (TreeA * HeapA)) 
-  : Tick (T HeapA) :=
-  match d with
-  | Some (tD, hpD) =>
-    let+ trsD := removeMinAuxD (trees hp) (Some (Thunk tD, treesA hpD)) in
-      Tick.ret (Thunk (MkHeapA trsD))
-  | None =>
-    let+ trsD := removeMinAuxD (trees hp) None in
-      Tick.ret (Thunk (MkHeapA trsD))
-  end.
-
-Definition valid_Tree (t : Tree) : Prop.
+  induction ts, outD.
+  - split; constructor; auto.
+  - inversion 1. repeat constructor; auto.
+  (* Impossible case. *)
+  - destruct (insTree_is_cons t (a :: ts)) as [ w [ x y ] ]. rewrite y. inversion 1.
+  - inversion 1. simpl. destruct (rank t <? rank a).
+    + inversion H2. subst. split. unfold strictD. simpl. destruct x1.
+      * constructor. inversion_clear H3.
 Admitted.
 
-Fixpoint valid_Trees (r : nat) (ts : list Tree) : Prop :=
-  match ts with
-  | nil => True
-  | t :: ts => valid_Tree t /\ r <= rank t /\ valid_Trees (S (rank t)) ts
-  end.
-
-Definition valid_Heap (h : Heap) : Prop := valid_Trees 0 (trees h).
-
-Definition max_rank (xs : list Tree) : nat.
-Admitted.
-
-(* number of zeros in the binary representation of xs *)
-Definition zbitcount (xs : list Tree) : nat :=
-  max_rank xs - length xs.
-
-Definition pot_heap h := zbitcount (trees h).
-
-Definition pot_heapA (h : HeapA) : nat.
-Admitted.
-
-Inductive less_defined_TreeA : TreeA -> TreeA -> Prop :=
-| ld_node : forall n1 n2 x1 x2 ts1 ts2,
-    less_defined n1 n2 ->
-    less_defined x1 x1 ->
-    less_defined ts1 ts2 ->
-    less_defined_TreeA (NodeA n1 x1 ts1) (NodeA n2 x2 ts2).
-#[global] Instance LessDefined_TreeA : LessDefined TreeA := less_defined_TreeA.
-
-#[global] Instance Exact_Tree : Exact Tree TreeA :=
-  fun t => match t with
-           | Node n x t => NodeA (exact n) (exact x) (exact t)
-           end.
-
-Lemma link_approx (t1 t2 : Tree) (outD : TreeA)
-  : outD `is_approx` link t1 t2 ->
-    Tick.val (linkD t1 t2 outD) `is_approx` (t1, t2).
-Proof.
-  remember (link t1 t2) as tlink. remember (exact tlink) as Texact.
-  destruct 1 as [n1 n2 x1 x2 ts1 ts2 Hn Hx Hts].
-  unfold exact. unfold AO_Exact. simpl. unfold Exact_Tree; constructor; simpl.
-  destruct t1, t2, ts1; simpl; destruct (Nat.leb_spec n0 n4).
-  destruct x. simpl. constructor. unfold less_defined.
-  unfold exact. unfold AO_Exact.
-Admitted.
-
-  (* destruct t1, t2. simpl. destruct (Nat.leb_spec n0 n4). t1; simpl. destruct x. simpl. *)
-
-
-  (* destruct t1, t2, 1. simpl. destruct (Nat.leb_spec n0 n2), ts1; constructor; simpl; try (destruct x); simpl; auto. *)
-  (* constructor. *)
-
-  (* intros. unfold less_defined in *. destruct H. *)
-  (* destruct t1 as [n1 x1 ts1], t2 as [n2 x2 ts2]. *)
-  (* destruct 1 as [na1 na2 xa1 xa2 ta1 ta2 Hna Hxa Htas]. *)
-  (* unfold linkD. destruct (Nat.leb_spec x1 x2); split. unfold TConsD. destruct ta1. destruct x. simpl. *)
-
-
-
-Definition less_defined_HeapA (h1 h2 : HeapA) : Prop := less_defined (treesA h1) (treesA h2).
-#[global] Instance LessDefined_HeapA : LessDefined HeapA := less_defined_HeapA.
-
-#[global] Instance Exact_HeapA : Exact Heap HeapA := fun h => MkHeapA (exact (trees h)).
-
-Definition measureT {a : Type} (f : a -> nat) (t : T a) : nat :=
-  match t with
-  | Undefined => 0
-  | Thunk x => f x
-  end.
-
-(*
-out = insert x inp
-cost (insertD x inp ..) <= zbitcount out - zbitcount inp
-*)
-
-Theorem cost_insert : forall x h d, d `is_approx` insert x h ->
-  forall xD hD, (xD, hD) = Tick.val (insertD x h d) ->
-  measureT pot_heapA hD + Tick.cost (insertD x h d) <= 1 + pot_heapA d.
-Proof.
-Admitted.
-
-Definition findMin (hp : Heap)
-  : option A :=
-  match removeMinTree hp with
-  | None => None
-  | Some (t, _) => Some (root t)
-  end.
-
-Definition findMinD (hp : Heap) (d : option A) : Tick (T HeapA) :=
-  match d with
-  | Some n => 
-    let t := NodeA Undefined (Thunk n) Undefined in
-    let+ hpD := removeMinTreeD hp (Some (t, MkHeapA Undefined)) in
-    Tick.ret hpD
-  | None => Tick.ret (Undefined)
-  end.
-
-Definition deleteMin (hp : Heap)
-  : Heap :=
-  match removeMinTree hp with
-  | None => MkHeap []
-  | Some (Node r v c, ts) =>
-    merge (MkHeap (rev c)) ts
-  end.
-
-Definition deleteMinD (hp : Heap) (d : HeapA) : Tick (T HeapA) :=
-  match removeMinTree hp with
-  | None => removeMinTreeD hp None
-  | Some (Node r v c, ts) =>
-    let+ (hpM1, hpM2) := mergeD (MkHeap (rev c)) ts d in
-    (*TODO: rev is strict*)
-    let ts := thunkD treesA hpM1 in
-    let hpM1' := NodeA (Thunk r) (Thunk v) ts in
-    removeMinTreeD hp (thunkD (H := None) (fun y => Some (hpM1', y)) hpM2)
-  end. (*TODO: is None correct for H*)
-
-
-(*
-(* Potential: number of trees
-   (times an implementation-dependent multiplicative factor)
-   It would be 1 if we just counted calls to [link].  *)
-3 
-Definition pot_heap (h : Heap) : T HeapA -> nat :=
-  measureT (fun _ => pot_trees (trees h)).
-
-(*
-  F : A -> B
-  DF : A -> B -> A
-
-  pot1 : B -> nat
-  pot2 : A -> nat
-
-  COST[DF a b] + pot1(DF a b) <= pot2(b) + constant
-*)
-
-Definition OTick_has_cost {A' : Type} (m : nat) (u : OTick A') (pre : A' -> nat) (post : nat) :=
-  match u with
-  | None => False
-  | Some v => m + pre (Tick.val v) + Tick.cost v <= post
-  end.
-
-Definition has_cost_ {A B : AA} {a : A} {b : B}
-    (f : DF a b) (m : nat) (pre : approx A -> nat) (post : approx B -> nat) (n : nat)
-  : Prop :=
-  forall b' : approx B, b' `is_approx` b ->
-    OTick_has_cost m (apply f b') pre (n + post b').
-
-Definition has_cost {A B : AA} {a : A} {b : B}
-    (f : DF a b) (pre : approx A -> nat) (post : approx B -> nat) (n : nat)
-  : Prop :=
-  has_cost_ f 0 pre post n.
-
-Definition measure_plus {A B : Type} (f : A -> nat) (g : B -> nat) (xy : A * B) : nat :=
-  f (fst xy) + g (snd xy).
-
-Infix "+++" := measure_plus (at level 40).
-
-Definition zero {A : Type} (_ : A) : nat := 0.
-
-(* Amortized complexity of insert *)
-Definition insert_budget := 3.
-
-Class Subadditive {A : AA} (f : approx A -> nat) : Prop :=
-  { subadditive_zero : forall x, f (bottom_of x) = 0
-  ; subadditive_lub  : forall x y, f (lub x y) <= f x + f y
-  }.
-
-#[global]
-Instance Subadditive_zero {A : AA} : Subadditive (A := A) zero.
-Proof.
-  constructor; reflexivity.
-Qed.
-
-#[global]
-Instance Subadditive_measure_plus {A B : AA}
-    (f : approx A -> nat) (g : approx B -> nat)
-    `(!Subadditive f, !Subadditive g)
-  : Subadditive (f +++ g).
-Proof.
-  constructor.
-  - intros []; unfold measure_plus; cbn.
-    rewrite 2 subadditive_zero. reflexivity.
-  - intros x y. unfold measure_plus; cbn.
-    rewrite 2 subadditive_lub. lia.
-Qed.
-
-#[global] Instance Proper_S_le : Proper (le ==> le) S.
-Proof. exact le_n_S. Qed.
-
-Lemma subadditive_sizeX' {a : Type} (n : nat) (xs ys : listA a)
-  : sizeX' n (lub xs ys) <= sizeX' n xs + sizeX' n ys.
-Proof.
-  revert ys; induction xs as [ | x | x xs IH ]; intros [| y [] ]; cbn; try rewrite IH; lia.
-Qed.
-
-(*
-#[global]
-Instance Subadditive_pot_heap : Subadditive (A := AA_Heap) pot_heap.
-Proof.
-  constructor.
-  - admit.
-  - admit.
-Admitted.
-*)
-
-Lemma let_cost {A B C : AA} {a : A} {b : B} {c : C} {f : DF a b} {g : DF (a, b) c}
-    {pre : approx A -> nat}
-    `{!Subadditive pre}
-    (mid : approx B -> nat) (post : approx C -> nat) (m0 m n : nat)
-    (_ : has_cost_ f m0 pre mid m)
-    (_ : has_cost_ g m (pre +++ mid) post n)
-  : has_cost_ (DF.let_ f g) m0 pre post n.
-Proof.
-  unfold DF.let_.
-Admitted.
-
-(*
-  f : G -> A
-
-  g : G * A -> B
-
-  n + post b'
-  >=
-  m + cost (g' b') + pre (fst (g' b')) + mid (snd (g' b'))
-  >=
-  m0 + cost (g' b') + cost (f' ...) + pre (fst (g' b')) + pre (f' ...)
-  >=
-  m0 + cost ... + pre (lub (fst (g' b')) (f' ...))
-*)
-
-Lemma tick_cost {A B : AA} {a : A} {b : B} (f : DF a b)
-    m pre post n
-  : has_cost_ f (S m) pre post n ->
-    has_cost_ (DF.tick f) m pre post n.
-Admitted.
-
-Lemma match_list_nil_cost {G A B : AA} {P : list A -> B} {g : G}
-    `{!AutoDF g []}
-    (NIL : DF (g, []) (P []))
-    (CONS : forall x ys, DF (g, x :: ys, x, ys) (P (x :: ys)))
-    m pre post n
-  : has_cost_ NIL m (pre +++ zero) post n ->
-    has_cost_ (match_list (var []) NIL CONS) m pre post n.
-Admitted.
-
-Definition measure_list_uncons {A  : AA} (x : A) (xs : list A) pot0 pot_hd pot_tl : Prop
-  := forall (x' : approx A) (xs' : approx (AA_listA A)), x' `is_approx` x -> xs' `is_approx` xs ->
-      pot0 (Thunk (ConsA (Thunk x') xs')) <= pot_hd + pot_tl xs'.
-
-Lemma match_list_cons_cost {G A B : AA} {P : list A -> B} {g : G} (x : A) (xs : list A)
-    `{!AutoDF g (x :: xs)}
-    (NIL : DF (g, []) (P []))
-    (CONS : forall x ys, DF (g, x :: ys, x, ys) (P (x :: ys)))
-    m pre pot0 m' pot_hd pot_tl post n
-  : has_cost_ (var (g := g) (x :: xs)) m pre pot0 m' ->
-    measure_list_uncons x xs pot0 pot_hd pot_tl ->
-    has_cost_ (CONS x xs) (m + pot_hd) (((pre +++ pot0) +++ zero) +++ pot_tl) post n ->
-    has_cost_ (match_list (var (x :: xs)) NIL CONS) m pre post n.
-Admitted.
-
-(*
-Lemma pot_trees_uncons (r : nat) (t : Tree) (ts : list Tree)
-  : valid_Trees r (t :: ts) ->
-    measure_list_uncons t ts (pot_trees r (t :: ts)) (rank t - r) (pot_trees (S (rank t)) ts).
-Proof.
-Admitted.
-*)
-
-Lemma consD_cost {G : AA} {g : G} {r : nat} {x : Tree} {xs : list Tree}
-    {xD : DF g x} {xsD : DF g xs} {m pre n}
-    `{!Subadditive pre}
-  : valid_Trees r (x :: xs) ->
-    m <= n + rank x - r ->
-    has_cost_ xD 0 pre zero 0 ->
-    has_cost_ xsD 0 pre zero (pot_trees xs - r) ->
-    has_cost_ (consD xD xsD) m pre zero (pot_trees (x :: xs) - r).
-Admitted.
-
-(*
-Lemma nilD_cost {G : AA} {g : G} {pre n} {r}
-    `{!Subadditive pre}
-  : has_cost_ (a := g) nilD 0 pre zero (pot_trees []).
-Proof.
-Admitted.
-*)
-
-Lemma has_cost_id {A : AA} {x : A} p n : has_cost_ (DF.id x) n p p n.
-Proof.
-  unfold has_cost_, DF.id; cbn. lia.
-Qed.
-
-Lemma has_cost_compose {A B C : AA} {x : A} {y : B} {z : C}
-  (f : DF x y) (g : DF y z) nf ng n pf pg p
-  : has_cost_ f nf pf pg ng ->
-    has_cost_ g ng pg p n ->
-    has_cost_ (f >>> g) nf pf p n.
-Proof.
-  unfold has_cost_, DF.compose, DF.Raw_compose; cbn.
-  intros Hf Hg z' Az.
-Admitted.
-
-Existing Class has_cost_.
-#[global]
-Hint Mode has_cost_ ! ! ! ! ! - - - - : typeclass_instances.
-
-#[global]
-Instance has_cost_autoDF_id {A : AA} {x : A} p
-  : has_cost_ (autoDF (x := x) (y := x)) 0 p p 0.
-Proof.
-  unfold autoDF, AutoDF_id. apply has_cost_id.
-Qed.
-
-Lemma has_cost_proj1 {A B : AA} {x : A} {y : B} n p q
-  : has_cost_ (DF.proj1 (x := x) (y := y)) n (p +++ q) p n.
-Proof.
-Admitted.
-
-Lemma has_cost_proj2 {A B : AA} {x : A} {y : B} n p q
-  : has_cost_ (DF.proj2 (x := x) (y := y)) n (p +++ q) q n.
-Proof.
-Admitted.
-
-#[global]
-Instance has_cost_autoDF_proj1 {A B C : AA} {x : A} {y : B} {z : C} `{!AutoDF x z} {p q r}
-  : has_cost_ (autoDF (x := x) (y := z)) 0 p r 0 ->
-    has_cost_ (autoDF (x := (x, y)) (y := z)) 0 (p +++ q) r 0.
-Proof.
-  unfold autoDF at 2, AutoDF_fst.
-  intros H.
-  eapply has_cost_compose.
-  - apply has_cost_proj1.
-  - apply H.
-Qed.
-
-#[global]
-Instance has_cost_autoDF_proj2 {A B : AA} {x : A} {y : B} {p q}
-  : has_cost_ (autoDF (x := (x, y)) (y := y)) 0 (p +++ q) q 0.
-Proof.
-  apply has_cost_proj2.
-Qed.
-
-#[global]
-Instance has_cost_pair {A B C : AA} {x : A} {y : B} {z : C} {p q r}
-    (f : DF x y) (g : DF x z)
-  : has_cost_ f 0 p q 0 ->
-    has_cost_ g 0 p r 0 ->
-    has_cost_ (DF.pair f g) 0 p (q +++ r) 0.
-Proof.
-Admitted.
-
-#[global]
-Instance has_cost_autoDF_pair {A B C : AA} {x : A} {y : B} {z : C} {p q r}
-    `{!AutoDF x y, !AutoDF x z}
-  : has_cost_ (autoDF (x := x) (y := y)) 0 p q 0 ->
-    has_cost_ (autoDF (x := x) (y := z)) 0 p r 0 ->
-    has_cost_ (autoDF (x := x) (y := (y, z))) 0 p (q +++ r) 0.
-Proof.
-  apply has_cost_pair.
-Qed.
-
-Lemma var_cost {G A : AA} {g : G} {x : A} `{!AutoDF g x} {pre post}
-    {Hauto : has_cost_ (autoDF (x := g) (y := x)) 0 pre post 0}
-  : has_cost_ (var (g := g) x) 0 pre post 0.
-Proof.
-  exact Hauto.
-Qed.
-
-Lemma weaken_cost {G A : AA} (g : G) (x : A) (f : DF g x) m pre post n
-  : m <= n ->
-    has_cost_ f 0 pre post 0 ->
-    has_cost_ f m pre post n.
-Proof.
-Admitted.
-
-Lemma call_cost {G1 G2 A : AA} {g1 : G1} {g2 : G2} {x : A} `{!AutoDF g2 g1}
-    {f : DF g1 x} {pre1 pre2 post n m}
-    {Hauto : has_cost_ (autoDF (x := g2) (y := g1)) 0 pre2 pre1 0}
-  : has_cost_ f n pre1 post m ->
-    has_cost_ (call (g1 := g1) (g2 := g2) f) n pre2 post m.
-Proof.
-  unfold call.
-  intros H. eapply has_cost_compose.
-  - eapply weaken_cost; [ reflexivity | ].
-    exact Hauto.
-  - apply H.
-Qed.
-
-Lemma if_cost {G A : AA} {g : G} {b : bool} {P : bool -> A}
-    (CASE : DF g b)
-    (TRUE : DF g (P true))
-    (FALSE : DF g (P false))
-    m n p q
-  : has_cost_ CASE 0 p zero 0 ->
-    (b = true -> has_cost_ TRUE m p q n) ->
-    (b = false -> has_cost_ FALSE m p q n) ->
-    has_cost_ (DF.if_ CASE TRUE FALSE) m p q n.
-Proof.
-Admitted.
-
-Theorem insTree_cost (t : Tree) (ts : list Tree)
-  : valid_Tree t ->
-    valid_Trees (rank t) ts ->
-    has_cost_ (insTreeDF t ts) (pot_trees ts) (zero +++ zero) zero (pot_trees (insTree t ts)).
-Proof.
-Admitted. (*
-  revert t; induction ts as [ | u ts IH]; intros t Vt Vts.
-  - cbn [insTreeDF].
-    apply tick_cost.
-    apply match_list_nil_cost.
-    apply consD_cost.
-    + split; [ | split]; [ assumption | lia | exact I].
-    + admit.
-    + apply var_cost.
-    + eapply weaken_cost. { unfold insert_budget; lia. }
-      apply nilD_cost.
-  - cbn [insTreeDF].
-    apply tick_cost.
-    eapply match_list_cons_cost with (pot0 := pot_trees (rank t) (u :: ts)) (pot_tl := pot_trees (S (rank u)) ts) (m' := S (rank t)).
-    + apply weaken_cost. { reflexivity. }
-      apply var_cost.
-    + apply pot_trees_uncons. assumption.
-    + apply let_cost with (mid := zero) (m := S (rank t) + (rank u - rank t)).
-      { apply call_cost. admit. }
-      apply let_cost with (mid := zero) (m := S (rank t) + (rank u - rank t)).
-      { apply call_cost. admit. }
-      apply let_cost with (mid := zero) (m := S (rank t) + (rank u - rank t)).
-      { apply call_cost. admit. }
-      refine (if_cost _ _ _ _ _ _ _ _ _ _).
-      * intros Htrue.
-        cbn [insTree]. rewrite Htrue.
-        assert (Vts' : valid_Trees (S (rank t)) (u :: ts)).
-        { admit. }
-        assert (Vtts' : valid_Trees 0 (t :: u :: ts)).
-        { admit. }
-        apply consD_cost.
-        { assumption. }
-        { admit. }
-        { exact _.  }
-        { apply consD_cost.
-          { assumption. }
-          { lia. }
-          { exact _. }
-          { eapply weaken_cost. cbn. lia. apply var_cost. } }
-      * intros Hfalse.
-        apply let_cost with (mid := zero) (m := 1 + (rank u - r)).
-        { apply call_cost. admit. }
-        apply call_cost.
-        eapply weaken_cost.
-Qed.
-*)
-
-Lemma nodeD_cost_zero {r : AA} {s : r} {n x : nat} {ts : list Tree}
-    {pre : approx r -> nat}
-    `{!Subadditive pre}
-    (nD : DF s n) (xD : DF s x) (tsD : DF s ts)
-  : has_cost_ nD 0 pre zero 0 ->
-    has_cost_ xD 0 pre zero 0 ->
-    has_cost_ tsD 0 pre zero 0 ->
-    has_cost_ (nodeD nD xD tsD) 0 pre zero 0.
-Proof.
-Admitted.
-
-Theorem insert_cost (x : A) (h : Heap)
-  : valid_Heap h ->
-    has_cost_ (insertDF x h) 0 (zero +++ zero) zero insert_budget.
-Proof. (*
-  intros Vh.
-  change insert_budget with (0 + insert_budget).
-  apply let_cost with (mid := zero) (m := 0); [ admit | |].
-  { apply nodeD_cost_zero.
-    + admit.
-    + admit.
-    + admit. }
-  change insert_budget with (0 + insert_budget).
-  apply let_cost with (mid := zero) (m := 0); [ admit | |].
-  { admit. }
-  assert (HH : has_cost_ (insTreeDF (Node 0 x []) (trees h)) 0 (zero +++ pot_list) pot_list insert_budget).
-  { apply insTree_cost. assumption. }
-  admit. *)
-Admitted.
-
-(*
-Below: TODO
-*)
-
-Canonical AA_comparison : ApproxAlgebra := exact_AA comparison.
-
-Definition DF_compare {G A : ApproxAlgebra} {g : G} {b : comparison} {P : comparison -> A}
-  : DF g b -> DF g (P Lt) -> DF g (P Eq) -> DF g (P Gt) -> DF g (P b) :=
-  (* TODO: use first argument *)
-  match b with
-  | Lt => fun _ p _ _ => p
-  | Eq => fun _ _ p _ => p
-  | Gt => fun _ _ _ p => p
-  end.
-
-Parameter compare_ : forall x y : nat, DF (x, y) (Nat.compare x y).
-
-Fixpoint mergeAuxDF (trs1 trs2 : list Tree) : DF (trs1, trs2) (mergeAux trs1 trs2) :=
-  match_list (P := fun trs1 => mergeAux trs1 trs2) (var trs1)
-    (var trs2)
-    (fun t1 trs1' =>
-      let trs1_ := t1 :: trs1' in
-      let fix merge_trs1DF trsR : DF (t1 :: trs1', t1, trs1', trsR) (mergeAux trs1_ trsR) :=
-        match_list (P := fun trsR => mergeAux trs1_ trsR) (var trsR)
-        (var trs1_)
-        (fun t2 trs2' =>
-          let trsR_ := t2 :: trs2' in
-          DF.let_ (call (rankDF t1))
-          (DF.let_ (call (rankDF t2)) 
-          (DF.let_ (call (compare_ (rank t1) (rank t2)))
-          (DF_compare (P := fun b => match b with Eq => _ | Lt => _ | Gt => _ end)
-             (var (Nat.compare (rank t1) (rank t2)))
-             (DF.let_ (call (mergeAuxDF trs1' trsR_))
-              (consD (var t1) (call (mergeAuxDF trs1' trsR_))))
-              (DF.let_ (call (linkDF t1 t2))
-                (DF.let_ (call (mergeAuxDF trs1' trs2'))
-                (DF.let_ (call (insTreeDF (link t1 t2) (mergeAux trs1' trs2')))
-                (call (insTreeDF (link t1 t2) (mergeAux trs1' trs2'))))))
-              (consD (var t2) (call (merge_trs1DF trs2')))))))
-      in
-      call (merge_trs1DF trs2)).
-
-Definition mergeDF (hp1 hp2 : Heap) : DF (hp1, hp2) (merge hp1 hp2) :=
-  DF.let_ (treesD (var hp1)) 
-  (DF.let_ (treesD (var hp2))
-  (MkHeapD (call (mergeAuxDF _ _)))).
-
-Fixpoint removeMinAux (ts : list Tree) : option (Tree * list Tree) := 
-  match ts with
-  | [] => None
-  | t :: ts' => match removeMinAux ts' with
-    | None => Some (t, [])
-    | Some (t', ts'') => if leb (root t) (root t')
-      then Some (t, ts')
-      else Some (t', t :: ts'')
-    end
-  end.
-
-Canonical AA_optionA (a : AA) : AA :=
-  {| carrier := option a
-  ;  approx := T (option (approx a))
-  ; AA_IsAA := TODO
-  ; AA_IsAS := TODO
-  ; AA_Setoid := TODO
-  |}.
-
-Definition noneD {G a : AA} {g : G} : DF g (None (A := a)).
-Admitted.
-  
-Definition someD {G A : AA} {g : G} {x : A}
-  : DF g x -> DF g (Some x).
-Admitted.
-
-(* Auxiliary definition for match_option *)
-Definition force_some {G A : AA} {g : G} {x : A}
-  : DF (g, (Some x)) (g, x).
-Admitted.
-
-Definition match_option {G A B : AA} {P : option A -> B} {g : G} {xO : option A}
-    (CASE : DF g xO)
-    (NONE : DF g (P None))
-    (SOME : forall x, DF (g, x) (P (Some x)))
-  : DF g (P xO) :=
-  DF.bind CASE
-  match xO with
-  | None => DF.proj1 >>> NONE
-  | Some x => force_some >>> SOME x
-  end.
-
-Fixpoint removeMinAuxDF (ts : list Tree) : DF ts (removeMinAux ts).
-Admitted. (* match_list (P := fun ts => removeMinAux ts) (var ts)
-  noneD
-  (fun t ts' => 
-    DF.let_ (call (removeMinAuxDF ts'))
-    (match_option (P 
-      (someD (DF.pair (var t) nilD))
-      (fun p => 
-        DF.let_ (call (rootDF t))
-        (DF.let_ (DF.proj1 >>> call (rootDF _))
-        (DF.let_ (DF.proj1 >>> call (lt_ (root _) (root t)))
-          (DF.if_ (P := fun b => if b then _ else _)
-            (DF.proj1 >>> var (root _ <? root t))
-            (someD (DF.pair (DF.proj1) (DF.proj2 >>> consD (var t) _)))
-            (someD (DF.pair (var t) (var ts')))))))
-    )).*)
-
-Definition heapConvert (p : Tree * (list Tree)) : (Tree * Heap) :=
-  match p with
-  | (t, ts) => (t, MkHeap ts)
-  end.
-
-Definition heapConvertDF (p : Tree * (list Tree)) : DF p (heapConvert p).
-Admitted.
-
-Definition removeMinTree (hp : Heap) 
-  : option ((Tree) * (Heap)) :=
-  match removeMinAux (trees hp) with
-  | Some (t, ts) => Some (t, MkHeap ts)
-  | None => None
-  end.
-
-(*Definition mergeDF (hp1 hp2 : Heap) : DF (hp1, hp2) (merge hp1 hp2) :=
-  DF.let_ (treesD (var hp1)) 
-  (DF.let_ (treesD (var hp2))
-  (MkHeapD (call (mergeAuxDF _ _)))).*)
-  
-(*Definition bind `{x : a, y : b, z : c} `(f : DF x y) `(g : DF (x, y) z) : DF x z :=
-  pair (id x) f >>> g.*)
-
-(*Definition treesD {G : AA} {g : G} {h : Heap} (f : DF g h) : DF g (trees h).*)
-
-(*Definition match_option {G A B : AA} {P : option A -> B} {g : G} {xO : option A}
-    (CASE : DF g xO)
-    (NONE : DF g (P None))
-    (SOME : forall x, DF (g, x) (P (Some x)))
-  : DF g (P xO) :=*)
-
-(*
-Definition var {G A : AA} {g : G} (x : A) `{AutoDF _ _ g x} : DF g x := autoDF.
-Definition call {x : A} `{AutoDF _ _ g2 g1} (f : DF g1 x)
-  : DF g2 x := autoDF >>> f.*)
-
-
-(*Fixpoint removeMinAuxDF (ts : list Tree) : DF ts (removeMinAux ts).
-
-Definition someD {G A : AA} {g : G} {x : A}
-  : DF g x -> DF g (Some x).*)
-
-Definition removeMinTreeDF (hp : Heap) : DF hp (removeMinTree hp).
-Admitted.
-  (*DF.let_ 
-  (treesD (var hp))
-
-  (*(g: DF (hp, trees hp) (removeMinTree hp))*)
-
-  (DF.let_
-    (*(f : DF (hp, trees hp) (removeMinAux ts))*) (call (removeMinAuxDF _))
-    (*(g : DF ((hp, trees hp), (removeMinAux ts)) (removeMinTree hp))*)
-    (match_option {P := fun h => removeMinAux h}
-      (*(CASE : DF ((hp, trees hp), (removeMinAux ts)) (removeMinAux ts))*)
-      (var (removeMinAux (trees hp)))
-      (*(NONE: DF ((hp, trees hp), (removeMinAux ts)) (P None))*)
-      noneD
-      (*(SOME: forall x, DF (((hp, trees hp), (removeMinAux ts)), x) (P (Some x))))*)
-      (fun p => someD (call (heapConvertDF p)))
-    )).*)
-(*  (DF.let_ (call (removeMinAuxDF _))
-  (match_option (var (removeMinAux ts)) 
-  noneD
-  (fun p => someD (DF.pair (DF.proj1) (DF.proj2 >>> MkHeapD _)))).*)
-
-Definition findMin (hp : Heap)
-  : option A :=
-  match removeMinTree hp with
-  | None => None
-  | Some (t, _) => Some (root t)
-  end.
-
-Definition findMinDF (hp : Heap) : DF hp (findMin hp).
-Admitted. (* :=
-  DF.let_ (call (removeMinTreeDF hp))
-  (match_option (var _)
-    noneD
-    (fun p => DF.proj1 >>> 
-      DF.let_ (rootDF _)
-      (someD _))).*)
-
-Definition deleteMin (hp : Heap)
-  : Heap :=
-  match removeMinTree hp with
-  | None => MkHeap []
-  | Some (Node r v c, ts) =>
-    merge (MkHeap (rev c)) ts
-  end.
-
-Definition revDF {A : AA} (xs : list A) : DF xs (rev xs).
-Admitted.
-
-Definition deleteMinDF (hp : Heap) : DF hp (deleteMin hp).
-Admitted.
-(*removeMinTreeDF hp >>>
-  (match_option (var _)
-  (MkHeapD nilD)
-  (fun p => DF.proj1 >>>
-    match_Tree
-    _
-    (fun r1 v1 c1 => 
-      DF.let_ (revD c1) (DF.let_ (MkHeapD _) (mergeDF _ (DF.proj2)))))).*)
-  
-
-(*
-Canonical AABComparison : AA :=
-  {| carrier := comparison |}.
-
-Definition if_ {a b : AA} {x : a} {cond : bool}
-  {f : bool -> b}
-  (i : DF x cond)
-  (thn : DF x (f true))
-  (els : DF x (f false))
-  : DF x (f cond).
-Proof. refine TODO. Defined.  
-
-(* Encoding of [Nat.compare] *)
-Definition natCompare {a b : AA} {c : a} {x y : nat} 
-  {f : comparison -> b}
-  (nats : DF c (x, y))
-  (Lt_ : DF c (f Lt))
-  (Eq_ : DF c (f Eq))
-  (Gt_ : DF c (f Gt))
-  : DF c (f (Nat.compare x y)).
-Proof. refine TODO. Defined.
-
-Fixpoint mergeAuxDF (trs1 trs2 : list Tree) : DF (trs1, trs2) (mergeAux trs1 trs2).
-Proof.
-  refine ((TODO : DF (trs1, trs2) (trs2, trs1)) >>>
-    (match_list (f := fun trs => mergeAux trs trs2)
-    _ (fun t1 trs1' => _))).
-  - cbn. refine TODO.
-  - refine ((TODO: DF (trs2, t1, trs1') (t1, trs1', trs2)) >>>
-    match_list (f := fun trs => mergeAux _ trs)
-    _ (fun t2 trs2' => _)).
-    + cbn [mergeAux]. refine (consD TODO TODO).
-    + cbn [mergeAux]. refine (natCompare 
-      (f := fun c => match c with
-        | Lt => _
-        | Eq => _
-        | Gt => _
-        end)
-        _
-        _
-        _ 
-        _).
-        * refine TODO.
-        * refine TODO.
-        * refine TODO.
-        * refine TODO. 
-Defined.
-
-Definition merge (hp1 hp2 : Heap) : Heap :=
-  MkHeap (mergeAux (trees hp1) (trees hp2)).
-
-Definition mergeDF {hp1 hp2} : DF (hp1, hp2) (merge hp1 hp2).
-Proof.
-  refine (letDF (TODO >>> @treesD hp1) _).
-  refine (letDF (TODO >>> @treesD hp2) _).
-  refine (letDF (TODO >>> mergeAuxDF (trees hp1) (trees hp2)) _).
-  refine (proj2DF >>> MkHeapD _).
-Defined.
-
-Fixpoint removeMinAux (ts : list Tree) := 
-  match ts with
-  | [] => None
-  | t :: ts' => match removeMinAux ts' with
-    | None => Some (t, [])
-    | Some (t', ts'') => if leb (root t) (root t')
-      then Some (t, ts')
-      else Some (t', t :: ts'')
-    end
-  end.
-
-Canonical AAoption (a : AA) : AA :=
-  {| carrier := option a |}.
-
-(* Encoding of match on options *)
-Definition match_option {a b c : AA} {g : b} {f : option a -> c} {xM : option a}
-    (NONE : DF g (f None))
-    (SOME : forall x, DF (g, x) (f (Some x)))
-  : DF (g, xM) (f xM) :=
-  match xM with
-  | None => TODO >>> NONE
-  | Some x => TODO >>> (SOME x)
-  end.
-
-(* Encoding of None *)
-Definition noneD {a b : AA} {x : a} : DF x (None (A := b)).
-Proof. refine TODO. Defined.
-
-(* Encoding of (Some _) *)
-Definition someD {r a : AA} {s : r} {x : a} {xM : option a} (sD : DF s x)
-  : DF s (Some x).
-Proof. refine TODO. Defined.
-
-Fixpoint removeMinAuxDF {ts} : DF ts (removeMinAux ts).
-Proof.
-  refine (TODO >>> 
-    match_list (f := fun ts => removeMinAux ts) (g := ts) _ (fun t ts' => _)). (*TODO*)
-  - cbn. refine TODO.
-  - cbn. refine TODO.
-Defined.
-
-Definition removeMinTree (hp : Heap) 
-  : option ((Tree) * (Heap)) :=
-  match removeMinAux (trees hp) with
-  | Some (t, ts) => Some (t, MkHeap ts)
-  | None => None
-  end.
-
-Definition removeMinTreeDF {hp} : DF hp (removeMinTree hp).
-Proof.
-  refine (letDF (TODO >>> @treesD hp) _).
-  refine (letDF (TODO >>> removeMinAuxDF) _).
-  refine (TODO >>> match_option 
-    (f := fun pM => match pM with
-      | None => None
-      | Some (t, ts) => Some (t, MkHeap ts) 
-      end)
-    (g := hp) (*TODO*)
-    (xM := removeMinAux (trees hp))
-    _ (fun x => _)). 
-  - refine noneD.
-  - refine TODO. Unshelve. cbn. apply trees. assumption. (*TODO*)
-Defined.
-
-Definition findMin (hp : Heap)
-  : option A :=
-  match removeMinTree hp with
-  | None => None
-  | Some (t, _) => Some (root t)
-  end.
-
-Definition findMindDF {hp} : DF hp (findMin hp).
-Proof.
-  refine (TODO >>> match_option 
-    (f := fun pM => match pM with
-      | None => None
-      | Some (t, _) => Some (root t) 
-  end)
-  (g := hp) (*TODO*)
-  (xM := removeMinTree hp)
-  _ (fun x => _)). 
-  - refine noneD.
-  - refine TODO. (*TODO*)
-Defined.
-
-Definition deleteMin (hp : Heap)
-  : Heap :=
-  match removeMinTree hp with
-  | None => MkHeap []
-  | Some (Node r v c, ts) =>
-    merge (MkHeap (rev c)) ts
-  end.
-  
-Definition deleteMinDF {hp} : DF hp (deleteMin hp).
-Proof.
-  refine (TODO >>> match_option 
-    (f := fun pM => match pM with
-      | None => MkHeap []
-      | Some (Node r v c, ts) =>
-        merge (MkHeap (rev c)) ts
-    end)
-  (g := hp) (*TODO*)
-  (xM := removeMinTree hp)
-  _ (fun x => _)). 
-  - refine TODO.
-  - refine TODO. (*TODO*)
-Defined.*)
-*)
+(* Inductive TreeA : Type := *)
+(*   | NodeA : T nat -> T A -> T (listA TreeA) -> TreeA. *)
+
+(* Canonical AA_Tree := *)
+(*   {| carrier := Tree *)
+(*   ;  approx := TreeA *)
+(*   ;  AA_Setoid := TODO *)
+(*   ;  AA_IsAA := TODO *)
+(*   ;  AA_IsAS := TODO *)
+(*   |}. *)
+
+(* Record Heap : Type := MkHeap *)
+(*   { trees : list Tree }. *)
+
+(* Record HeapA : Type := MkHeapA *)
+(*   { treesA : T (listA TreeA) }. *)
+
+(* Canonical AA_Heap : AA := *)
+(*   {| carrier := Heap *)
+(*   ;  approx := T HeapA *)
+(*   ;  AA_Setoid := TODO *)
+(*   ;  AA_IsAA := TODO *)
+(*   ;  AA_IsAS := TODO *)
+(*   |}. *)
+
+(* Definition link (t1 t2 : Tree) : Tree := *)
+(*   match t1, t2 with *)
+(*   | Node r1 v1 c1, Node r2 v2 c2 => if leb v1 v2 *)
+(*     then Node (r1 + 1) v1 (t2 :: c1) *)
+(*     else Node (r2 + 1) v2 (t1 :: c2) *)
+(*   end. *)
+
+(* (* Encoding of Node *) *)
+(* (* Currently unused, just pattern-match on it instead *) *)
+(* Definition NodeD (t : TreeA) : Tick (T nat * T A * T (listA TreeA)) := *)
+(*   Tick.ret *)
+(*   match t with *)
+(*   | NodeA n x ts => (n, x, ts) *)
+(*   end. *)
+
+(* Definition TNodeD (t : T TreeA) : Tick (T nat * T A * T (listA TreeA)) := *)
+(*   Tick.ret *)
+(*   match t with *)
+(*   | Thunk (NodeA n x ts) => (n, x, ts) *)
+(*   | Undefined => (Undefined, Undefined, Undefined) *)
+(*   end. *)
+
+(* Definition ConsD {A} (xs : listA A) : T A * T (listA A) := *)
+(*   match xs with *)
+(*   | ConsA x ys => (x, ys) *)
+(*   | _ => (Undefined, Undefined) (* should not happen *) *)
+(*   end. *)
+
+(* Definition TConsD {A} (xs : T (listA A)) : T A * T (listA A) := *)
+(*   match xs with *)
+(*   | Thunk (ConsA x ys) => (x, ys) *)
+(*   | Undefined | _ => (Undefined, Undefined) *)
+(*   end. *)
+
+(* Definition linkD (t1 t2 : Tree) (d : TreeA) : Tick (T TreeA * T TreeA) := *)
+(*   match t1, t2 with *)
+(*   | Node r1 v1 c1, Node r2 v2 c2 => *)
+(*     if leb v1 v2 then *)
+(*       match d with *)
+(*       | NodeA rD v1D tsD => *)
+(*         let '(t2D, c1D) := TConsD tsD in *)
+(*         Tick.ret (Thunk (NodeA (exact r1) v1D c1D), t2D) *)
+(*       end *)
+(*     else *)
+(*       match d with *)
+(*       | NodeA rD v2D tsD => *)
+(*         let '(t1D, c2D) := TConsD tsD in *)
+(*         Tick.ret (t1D, Thunk (NodeA (exact r2) v2D c2D)) *)
+(*       end *)
+(*   end. *)
+
+(* (* Currently unused, just pattern-match *) *)
+(* Definition MkHeapD (d : HeapA) : Tick (T (listA TreeA)) := *)
+(*   Tick.ret (treesA d). *)
+
+(* Definition rank (t : Tree) : nat := *)
+(*   match t with *)
+(*   | (Node r v c) => r *)
+(*   end. *)
+
+(* Definition root (t : Tree) : A := *)
+(*   match t with *)
+(*   | (Node r v c) => v *)
+(*   end. *)
+
+(* (*Assumes t has rank <= the rank of the first element of ts (if any).*) *)
+(* Fixpoint insTree (t : Tree) (ts : list Tree) : list Tree := *)
+(*   match ts with *)
+(*   | [] => [t] *)
+(*   | t' :: ts' => if rank t <? rank t' *)
+(*     then t :: ts *)
+(*     else insTree (link t t') ts' (*t and t' should have the same rank*) *)
+(*   end. *)
+
+(* Definition strictD (t : Tree) (x' : T TreeA) : T TreeA := lub x' (Thunk (NodeA (exact (rank t)) Undefined Undefined)). *)
+(* Definition strictConsD {A} (xs' : T (listA A)) : T (listA A) := lub xs' (Thunk (ConsA Undefined Undefined)). *)
+
+(* (* [d] is an approximation of the output [insTree t ts] *) *)
+(* Fixpoint insTreeD (t : Tree) (ts : list Tree) (d : listA TreeA) : Tick (T TreeA * T (listA TreeA)) := *)
+(*   match ts with *)
+(*   | [] => *)
+(*     (* [d] is an approximation of [t :: nil] *) *)
+(*     (* ConsD inverts it and returns approximations of [t] and [nil] (which is ignored) *) *)
+(*     let '(tD, _) := ConsD d in *)
+(*     (* To find out what to return, we enumerate all of the uses of the arguments of [insTree]: *)
+(*        - [t] was only used in the output list, corresponding to the demand [tD] *)
+(*        - [ts] was used in [match], so its demand must at least be [Thunk NilA], which is fully defined. *)
+(*     *) *)
+(*     Tick.ret (tD, Thunk NilA) *)
+(*   | t' :: ts' => if rank t <? rank t' *)
+(*     then (* [d] is an approximation of [t :: ts] *) *)
+(*          let '(tD, tsD) := ConsD d in *)
+(*          (* [t] occurs in the result [t :: ts] (with demand [tD]), and also to compare its rank, *)
+(*             so we use [strictD] to give its demand a defined rank. *)
+(*             [ts] was also pattern-matched on, so we similarly require an annotation *)
+(*             to make its demand not [Undefined]. *) *)
+(*          Tick.ret (strictD t tD, strictConsD tsD) *)
+(*     else (* The result of [insTree] is a recursive call. So we recursively compute the *)
+(*             demand on its arguments: [lD] is the demand on [link t t'], and [ts'D] is the demand *)
+(*             on [ts]. *) *)
+(*          let+ (lD, ts'D) := insTreeD (link t t') ts' d in *)
+(*          (* [linkD] takes [lD] to compute a demand on [t] and [t']. *)
+
+(*             Demand functions return results wrapped in [T] (so that [Undefined] *)
+(*             may indicate an unused argument), but the input demand is not wrapped in [T] *)
+(*             (since there is no point in calling this if the argument is unused). *)
+(*             We use [thunkD] to apply a demand function on a demand wrapped in *)
+(*             [T] (here [lD]), usually coming from a pattern or another function. *) *)
+(*          let+ (tD, t'D) := thunkD (linkD t t') lD in *)
+(*          Tick.ret (strictD t tD, Thunk (ConsA t'D ts'D)) *)
+(*   end. *)
+
+(* Definition insert (x : A) (hp : Heap) *)
+(*   : Heap := *)
+(*   MkHeap (insTree (Node 0 x []) (trees hp)). *)
+
+(* Definition insertD (x : A) (hp : Heap) (d : HeapA) : Tick (T A * T HeapA) := *)
+(*   let+ (tD, trees_hpD) := thunkD (insTreeD (Node 0 x []) (trees hp)) (treesA d) in *)
+(*   let+ (_, xD, _) := TNodeD tD in *)
+(*   Tick.ret (xD, Thunk (MkHeapA trees_hpD)). *)
+
+
+(* Fixpoint mergeAux (trs1 trs2 : list Tree) : list Tree := *)
+(*   match trs1 with *)
+(*   | [] => trs2 *)
+(*   | t1 :: trs1' => let fix merge_trs1 trsR := *)
+(*     match trsR with *)
+(*     | [] => trs1 *)
+(*     | t2 :: trs2' => *)
+(*       match Nat.compare (rank t1) (rank t2) with *)
+(*       | Lt => t1 :: (mergeAux trs1' trsR) *)
+(*       | Eq => insTree (link t1 t2) (mergeAux trs1' trs2') *)
+(*       | Gt => t2 :: merge_trs1 trs2' *)
+(*       end *)
+(*     end in *)
+(*     merge_trs1 trs2 *)
+(*   end. *)
+
+(* Definition merge (hp1 hp2 : Heap) : Heap := *)
+(*   MkHeap (mergeAux (trees hp1) (trees hp2)). *)
+
+(* Fixpoint mergeAuxD (trs1 trs2 : list Tree) (d : listA TreeA) : Tick (T (listA TreeA) * T (listA TreeA)) := *)
+(*   match trs1 with *)
+(*   | [] => Tick.ret (Thunk NilA, Thunk d) *)
+(*   | t1 :: trs1' => let fix merge_trs1 trsR (dR : listA TreeA) : Tick (T (listA TreeA) * T (listA TreeA)) := *)
+(*     (* here we compute the demand on [trs1] and [trsR] *) *)
+(*     match trsR with *)
+(*     | [] => Tick.ret (Thunk dR, Thunk NilA) *)
+(*     | t2 :: trs2' => *)
+(*       match Nat.compare (rank t1) (rank t2) with *)
+(*       | Lt => *)
+(*         let '(t1D, mD) := ConsD dR in *)
+(*         let+ (trs1'D, trsRD) := thunkD (mergeAuxD trs1' trsR) mD in *)
+(*         Tick.ret (Thunk (ConsA (strictD t1 t1D) trs1'D), strictConsD trsRD) *)
+(*       | Eq => *)
+(*         let+ (lD, mD) := insTreeD (link t1 t2) (mergeAux trs1' trs2') dR in *)
+(*         let+ (t1D, t2D) := thunkD (linkD t1 t2) lD in *)
+(*         let+ (trs1'D, trs2'D) := thunkD (mergeAuxD trs1' trs2') mD in *)
+(*         Tick.ret (Thunk (ConsA (strictD t1 t1D) trs1'D), Thunk (ConsA (strictD t2 t2D) trs2'D)) *)
+(*       | Gt => *)
+(*         let '(t2D, mD) := ConsD dR in *)
+(*         let+ (trs1D, trs2'D) := thunkD (merge_trs1 trs2') mD in *)
+(*         Tick.ret (trs1D, Thunk (ConsA (strictD t2 t2D) trs2'D)) *)
+(*       end *)
+(*     end in *)
+(*     let+ (trs1D, trs2D) := merge_trs1 trs2 d in *)
+(*     Tick.ret (strictConsD trs1D, trs2D) *)
+(*   end. *)
+
+(* Definition mergeD (hp1 hp2 : Heap) (d : HeapA) : Tick (T HeapA * T HeapA) := *)
+(*   let+ (ts1D, ts2D) := thunkD (mergeAuxD (trees hp1) (trees hp2)) (treesA d) in *)
+(*   Tick.ret (Thunk (MkHeapA ts1D), Thunk (MkHeapA ts2D)). *)
+
+(* Fixpoint removeMinAux (ts : list Tree) : option (Tree * list Tree) := *)
+(*   match ts with *)
+(*   | [] => None *)
+(*   | t :: ts' => match removeMinAux ts' with *)
+(*     | None => Some (t, []) *)
+(*     | Some (t', ts'') => if leb (root t) (root t') *)
+(*       then Some (t, ts') *)
+(*       else Some (t', t :: ts'') *)
+(*     end *)
+(*   end. *)
+
+(* Definition SomeD {A} `{Bottom A} (x : option A) : A := *)
+(*   match x with *)
+(*   | Some y => y *)
+(*   | _ => bottom *)
+(*   end. *)
+
+(* Fixpoint removeMinAuxD (ts : list Tree) (d : option (T TreeA * T (listA TreeA))) *)
+(*   : Tick (T (listA TreeA)) := *)
+(*   match ts with *)
+(*   | [] => Tick.ret (Thunk NilA) *)
+(*   | t :: ts' => match removeMinAux ts' with *)
+(*     | None => *)
+(*       let (tD, _) := SomeD d in *)
+(*       let+ ts'D := removeMinAuxD ts' None in *)
+(*       Tick.ret (Thunk (ConsA tD ts'D)) *)
+(*     | Some (t', ts'') => if leb (root t) (root t') *)
+(*       then *)
+(*         let '(tD, ts'D) := SomeD d in *)
+(*         let+ ts'D := removeMinAuxD ts' (Some (strictD t' Undefined, Undefined)) in *)
+(*         Tick.ret (Thunk (ConsA tD ts'D)) *)
+(*       else *)
+(*         let '(t'D, tts''D) := SomeD d in *)
+(*         let '(tD, ts''D) := TConsD tts''D in *)
+(*         let+ ts'D := removeMinAuxD ts' (Some (strictD t' t'D, ts''D)) in *)
+(*         Tick.ret (Thunk (ConsA tD ts'D)) *)
+(*     end *)
+(*   end. *)
+
+(* Definition removeMinTree (hp : Heap) *)
+(*   : option ((Tree) * (Heap)) := *)
+(*   match removeMinAux (trees hp) with *)
+(*   | Some (t, ts) => Some (t, MkHeap ts) *)
+(*   | None => None *)
+(*   end. *)
+
+(* Definition removeMinTreeD (hp : Heap) (d : option (TreeA * HeapA))  *)
+(*   : Tick (T HeapA) := *)
+(*   match d with *)
+(*   | Some (tD, hpD) => *)
+(*     let+ trsD := removeMinAuxD (trees hp) (Some (Thunk tD, treesA hpD)) in *)
+(*       Tick.ret (Thunk (MkHeapA trsD)) *)
+(*   | None => *)
+(*     let+ trsD := removeMinAuxD (trees hp) None in *)
+(*       Tick.ret (Thunk (MkHeapA trsD)) *)
+(*   end. *)
+
+(* Definition valid_Tree (t : Tree) : Prop. *)
+(* Admitted. *)
+
+(* Fixpoint valid_Trees (r : nat) (ts : list Tree) : Prop := *)
+(*   match ts with *)
+(*   | nil => True *)
+(*   | t :: ts => valid_Tree t /\ r <= rank t /\ valid_Trees (S (rank t)) ts *)
+(*   end. *)
+
+(* Definition valid_Heap (h : Heap) : Prop := valid_Trees 0 (trees h). *)
+
+(* Definition max_rank (xs : list Tree) : nat. *)
+(* Admitted. *)
+
+(* (* number of zeros in the binary representation of xs *) *)
+(* Definition zbitcount (xs : list Tree) : nat := *)
+(*   max_rank xs - length xs. *)
+
+(* Definition pot_heap h := zbitcount (trees h). *)
+
+(* Definition pot_heapA (h : HeapA) : nat. *)
+(* Admitted. *)
+
+(* Inductive less_defined_TreeA : TreeA -> TreeA -> Prop := *)
+(* | ld_node : forall n1 n2 x1 x2 ts1 ts2, *)
+(*     less_defined n1 n2 -> *)
+(*     less_defined x1 x1 -> *)
+(*     less_defined ts1 ts2 -> *)
+(*     less_defined_TreeA (NodeA n1 x1 ts1) (NodeA n2 x2 ts2). *)
+(* #[global] Instance LessDefined_TreeA : LessDefined TreeA := less_defined_TreeA. *)
+
+(* #[global] Instance Exact_Tree : Exact Tree TreeA := *)
+(*   fun t => match t with *)
+(*            | Node n x t => NodeA (exact n) (exact x) (exact t) *)
+(*            end. *)
+
+(* Lemma link_approx (t1 t2 : Tree) (outD : TreeA) *)
+(*   : outD `is_approx` link t1 t2 -> *)
+(*     Tick.val (linkD t1 t2 outD) `is_approx` (t1, t2). *)
+(* Proof. *)
+(*   destruct 1 as [n1 n2 x1 x2 ts1 ts2 Hn Hx Hts]. *)
+(*   constructor; destruct t1, t2, ts1. simpl; destruct (Nat.leb_spec n0 n4), x. *)
+(*   constructor. unfold less_defined. *)
+(*   unfold exact. unfold AO_Exact. *)
+(* Admitted. *)
+
+(*   (* destruct t1, t2. simpl. destruct (Nat.leb_spec n0 n4). t1; simpl. destruct x. simpl. *) *)
+
+
+(*   (* destruct t1, t2, 1. simpl. destruct (Nat.leb_spec n0 n2), ts1; constructor; simpl; try (destruct x); simpl; auto. *) *)
+(*   (* constructor. *) *)
+
+(*   (* intros. unfold less_defined in *. destruct H. *) *)
+(*   (* destruct t1 as [n1 x1 ts1], t2 as [n2 x2 ts2]. *) *)
+(*   (* destruct 1 as [na1 na2 xa1 xa2 ta1 ta2 Hna Hxa Htas]. *) *)
+(*   (* unfold linkD. destruct (Nat.leb_spec x1 x2); split. unfold TConsD. destruct ta1. destruct x. simpl. *) *)
+
+
+
+(* Definition less_defined_HeapA (h1 h2 : HeapA) : Prop := less_defined (treesA h1) (treesA h2). *)
+(* #[global] Instance LessDefined_HeapA : LessDefined HeapA := less_defined_HeapA. *)
+
+(* #[global] Instance Exact_HeapA : Exact Heap HeapA := fun h => MkHeapA (exact (trees h)). *)
+
+(* Definition measureT {a : Type} (f : a -> nat) (t : T a) : nat := *)
+(*   match t with *)
+(*   | Undefined => 0 *)
+(*   | Thunk x => f x *)
+(*   end. *)
+
+(* (* *)
+(* out = insert x inp *)
+(* cost (insertD x inp ..) <= zbitcount out - zbitcount inp *)
+(* *) *)
+
+(* Theorem cost_insert : forall x h d, d `is_approx` insert x h -> *)
+(*   forall xD hD, (xD, hD) = Tick.val (insertD x h d) -> *)
+(*   measureT pot_heapA hD + Tick.cost (insertD x h d) <= 1 + pot_heapA d. *)
+(* Proof. *)
+(* Admitted. *)
+
+(* Definition findMin (hp : Heap) *)
+(*   : option A := *)
+(*   match removeMinTree hp with *)
+(*   | None => None *)
+(*   | Some (t, _) => Some (root t) *)
+(*   end. *)
+
+(* Definition findMinD (hp : Heap) (d : option A) : Tick (T HeapA) := *)
+(*   match d with *)
+(*   | Some n =>  *)
+(*     let t := NodeA Undefined (Thunk n) Undefined in *)
+(*     let+ hpD := removeMinTreeD hp (Some (t, MkHeapA Undefined)) in *)
+(*     Tick.ret hpD *)
+(*   | None => Tick.ret (Undefined) *)
+(*   end. *)
+
+(* Definition deleteMin (hp : Heap) *)
+(*   : Heap := *)
+(*   match removeMinTree hp with *)
+(*   | None => MkHeap [] *)
+(*   | Some (Node r v c, ts) => *)
+(*     merge (MkHeap (rev c)) ts *)
+(*   end. *)
+
+(* Definition deleteMinD (hp : Heap) (d : HeapA) : Tick (T HeapA) := *)
+(*   match removeMinTree hp with *)
+(*   | None => removeMinTreeD hp None *)
+(*   | Some (Node r v c, ts) => *)
+(*     let+ (hpM1, hpM2) := mergeD (MkHeap (rev c)) ts d in *)
+(*     (*TODO: rev is strict*) *)
+(*     let ts := thunkD treesA hpM1 in *)
+(*     let hpM1' := NodeA (Thunk r) (Thunk v) ts in *)
+(*     removeMinTreeD hp (thunkD (H := None) (fun y => Some (hpM1', y)) hpM2) *)
+(*   end. (*TODO: is None correct for H*) *)
+
+
+(* (* *)
+(* (* Potential: number of trees *)
+(*    (times an implementation-dependent multiplicative factor) *)
+(*    It would be 1 if we just counted calls to [link].  *) *)
+(* 3  *)
+(* Definition pot_heap (h : Heap) : T HeapA -> nat := *)
+(*   measureT (fun _ => pot_trees (trees h)). *)
+
+(* (* *)
+(*   F : A -> B *)
+(*   DF : A -> B -> A *)
+
+(*   pot1 : B -> nat *)
+(*   pot2 : A -> nat *)
+
+(*   COST[DF a b] + pot1(DF a b) <= pot2(b) + constant *)
+(* *) *)
+
+(* Definition OTick_has_cost {A' : Type} (m : nat) (u : OTick A') (pre : A' -> nat) (post : nat) := *)
+(*   match u with *)
+(*   | None => False *)
+(*   | Some v => m + pre (Tick.val v) + Tick.cost v <= post *)
+(*   end. *)
+
+(* Definition has_cost_ {A B : AA} {a : A} {b : B} *)
+(*     (f : DF a b) (m : nat) (pre : approx A -> nat) (post : approx B -> nat) (n : nat) *)
+(*   : Prop := *)
+(*   forall b' : approx B, b' `is_approx` b -> *)
+(*     OTick_has_cost m (apply f b') pre (n + post b'). *)
+
+(* Definition has_cost {A B : AA} {a : A} {b : B} *)
+(*     (f : DF a b) (pre : approx A -> nat) (post : approx B -> nat) (n : nat) *)
+(*   : Prop := *)
+(*   has_cost_ f 0 pre post n. *)
+
+(* Definition measure_plus {A B : Type} (f : A -> nat) (g : B -> nat) (xy : A * B) : nat := *)
+(*   f (fst xy) + g (snd xy). *)
+
+(* Infix "+++" := measure_plus (at level 40). *)
+
+(* Definition zero {A : Type} (_ : A) : nat := 0. *)
+
+(* (* Amortized complexity of insert *) *)
+(* Definition insert_budget := 3. *)
+
+(* Class Subadditive {A : AA} (f : approx A -> nat) : Prop := *)
+(*   { subadditive_zero : forall x, f (bottom_of x) = 0 *)
+(*   ; subadditive_lub  : forall x y, f (lub x y) <= f x + f y *)
+(*   }. *)
+
+(* #[global] *)
+(* Instance Subadditive_zero {A : AA} : Subadditive (A := A) zero. *)
+(* Proof. *)
+(*   constructor; reflexivity. *)
+(* Qed. *)
+
+(* #[global] *)
+(* Instance Subadditive_measure_plus {A B : AA} *)
+(*     (f : approx A -> nat) (g : approx B -> nat) *)
+(*     `(!Subadditive f, !Subadditive g) *)
+(*   : Subadditive (f +++ g). *)
+(* Proof. *)
+(*   constructor. *)
+(*   - intros []; unfold measure_plus; cbn. *)
+(*     rewrite 2 subadditive_zero. reflexivity. *)
+(*   - intros x y. unfold measure_plus; cbn. *)
+(*     rewrite 2 subadditive_lub. lia. *)
+(* Qed. *)
+
+(* #[global] Instance Proper_S_le : Proper (le ==> le) S. *)
+(* Proof. exact le_n_S. Qed. *)
+
+(* Lemma subadditive_sizeX' {a : Type} (n : nat) (xs ys : listA a) *)
+(*   : sizeX' n (lub xs ys) <= sizeX' n xs + sizeX' n ys. *)
+(* Proof. *)
+(*   revert ys; induction xs as [ | x | x xs IH ]; intros [| y [] ]; cbn; try rewrite IH; lia. *)
+(* Qed. *)
+
+(* (* *)
+(* #[global] *)
+(* Instance Subadditive_pot_heap : Subadditive (A := AA_Heap) pot_heap. *)
+(* Proof. *)
+(*   constructor. *)
+(*   - admit. *)
+(*   - admit. *)
+(* Admitted. *)
+(* *) *)
+
+(* Lemma let_cost {A B C : AA} {a : A} {b : B} {c : C} {f : DF a b} {g : DF (a, b) c} *)
+(*     {pre : approx A -> nat} *)
+(*     `{!Subadditive pre} *)
+(*     (mid : approx B -> nat) (post : approx C -> nat) (m0 m n : nat) *)
+(*     (_ : has_cost_ f m0 pre mid m) *)
+(*     (_ : has_cost_ g m (pre +++ mid) post n) *)
+(*   : has_cost_ (DF.let_ f g) m0 pre post n. *)
+(* Proof. *)
+(*   unfold DF.let_. *)
+(* Admitted. *)
+
+(* (* *)
+(*   f : G -> A *)
+
+(*   g : G * A -> B *)
+
+(*   n + post b' *)
+(*   >= *)
+(*   m + cost (g' b') + pre (fst (g' b')) + mid (snd (g' b')) *)
+(*   >= *)
+(*   m0 + cost (g' b') + cost (f' ...) + pre (fst (g' b')) + pre (f' ...) *)
+(*   >= *)
+(*   m0 + cost ... + pre (lub (fst (g' b')) (f' ...)) *)
+(* *) *)
+
+(* Lemma tick_cost {A B : AA} {a : A} {b : B} (f : DF a b) *)
+(*     m pre post n *)
+(*   : has_cost_ f (S m) pre post n -> *)
+(*     has_cost_ (DF.tick f) m pre post n. *)
+(* Admitted. *)
+
+(* Lemma match_list_nil_cost {G A B : AA} {P : list A -> B} {g : G} *)
+(*     `{!AutoDF g []} *)
+(*     (NIL : DF (g, []) (P [])) *)
+(*     (CONS : forall x ys, DF (g, x :: ys, x, ys) (P (x :: ys))) *)
+(*     m pre post n *)
+(*   : has_cost_ NIL m (pre +++ zero) post n -> *)
+(*     has_cost_ (match_list (var []) NIL CONS) m pre post n. *)
+(* Admitted. *)
+
+(* Definition measure_list_uncons {A  : AA} (x : A) (xs : list A) pot0 pot_hd pot_tl : Prop *)
+(*   := forall (x' : approx A) (xs' : approx (AA_listA A)), x' `is_approx` x -> xs' `is_approx` xs -> *)
+(*       pot0 (Thunk (ConsA (Thunk x') xs')) <= pot_hd + pot_tl xs'. *)
+
+(* Lemma match_list_cons_cost {G A B : AA} {P : list A -> B} {g : G} (x : A) (xs : list A) *)
+(*     `{!AutoDF g (x :: xs)} *)
+(*     (NIL : DF (g, []) (P [])) *)
+(*     (CONS : forall x ys, DF (g, x :: ys, x, ys) (P (x :: ys))) *)
+(*     m pre pot0 m' pot_hd pot_tl post n *)
+(*   : has_cost_ (var (g := g) (x :: xs)) m pre pot0 m' -> *)
+(*     measure_list_uncons x xs pot0 pot_hd pot_tl -> *)
+(*     has_cost_ (CONS x xs) (m + pot_hd) (((pre +++ pot0) +++ zero) +++ pot_tl) post n -> *)
+(*     has_cost_ (match_list (var (x :: xs)) NIL CONS) m pre post n. *)
+(* Admitted. *)
+
+(* (* *)
+(* Lemma pot_trees_uncons (r : nat) (t : Tree) (ts : list Tree) *)
+(*   : valid_Trees r (t :: ts) -> *)
+(*     measure_list_uncons t ts (pot_trees r (t :: ts)) (rank t - r) (pot_trees (S (rank t)) ts). *)
+(* Proof. *)
+(* Admitted. *)
+(* *) *)
+
+(* Lemma consD_cost {G : AA} {g : G} {r : nat} {x : Tree} {xs : list Tree} *)
+(*     {xD : DF g x} {xsD : DF g xs} {m pre n} *)
+(*     `{!Subadditive pre} *)
+(*   : valid_Trees r (x :: xs) -> *)
+(*     m <= n + rank x - r -> *)
+(*     has_cost_ xD 0 pre zero 0 -> *)
+(*     has_cost_ xsD 0 pre zero (pot_trees xs - r) -> *)
+(*     has_cost_ (consD xD xsD) m pre zero (pot_trees (x :: xs) - r). *)
+(* Admitted. *)
+
+(* (* *)
+(* Lemma nilD_cost {G : AA} {g : G} {pre n} {r} *)
+(*     `{!Subadditive pre} *)
+(*   : has_cost_ (a := g) nilD 0 pre zero (pot_trees []). *)
+(* Proof. *)
+(* Admitted. *)
+(* *) *)
+
+(* Lemma has_cost_id {A : AA} {x : A} p n : has_cost_ (DF.id x) n p p n. *)
+(* Proof. *)
+(*   unfold has_cost_, DF.id; cbn. lia. *)
+(* Qed. *)
+
+(* Lemma has_cost_compose {A B C : AA} {x : A} {y : B} {z : C} *)
+(*   (f : DF x y) (g : DF y z) nf ng n pf pg p *)
+(*   : has_cost_ f nf pf pg ng -> *)
+(*     has_cost_ g ng pg p n -> *)
+(*     has_cost_ (f >>> g) nf pf p n. *)
+(* Proof. *)
+(*   unfold has_cost_, DF.compose, DF.Raw_compose; cbn. *)
+(*   intros Hf Hg z' Az. *)
+(* Admitted. *)
+
+(* Existing Class has_cost_. *)
+(* #[global] *)
+(* Hint Mode has_cost_ ! ! ! ! ! - - - - : typeclass_instances. *)
+
+(* #[global] *)
+(* Instance has_cost_autoDF_id {A : AA} {x : A} p *)
+(*   : has_cost_ (autoDF (x := x) (y := x)) 0 p p 0. *)
+(* Proof. *)
+(*   unfold autoDF, AutoDF_id. apply has_cost_id. *)
+(* Qed. *)
+
+(* Lemma has_cost_proj1 {A B : AA} {x : A} {y : B} n p q *)
+(*   : has_cost_ (DF.proj1 (x := x) (y := y)) n (p +++ q) p n. *)
+(* Proof. *)
+(* Admitted. *)
+
+(* Lemma has_cost_proj2 {A B : AA} {x : A} {y : B} n p q *)
+(*   : has_cost_ (DF.proj2 (x := x) (y := y)) n (p +++ q) q n. *)
+(* Proof. *)
+(* Admitted. *)
+
+(* #[global] *)
+(* Instance has_cost_autoDF_proj1 {A B C : AA} {x : A} {y : B} {z : C} `{!AutoDF x z} {p q r} *)
+(*   : has_cost_ (autoDF (x := x) (y := z)) 0 p r 0 -> *)
+(*     has_cost_ (autoDF (x := (x, y)) (y := z)) 0 (p +++ q) r 0. *)
+(* Proof. *)
+(*   unfold autoDF at 2, AutoDF_fst. *)
+(*   intros H. *)
+(*   eapply has_cost_compose. *)
+(*   - apply has_cost_proj1. *)
+(*   - apply H. *)
+(* Qed. *)
+
+(* #[global] *)
+(* Instance has_cost_autoDF_proj2 {A B : AA} {x : A} {y : B} {p q} *)
+(*   : has_cost_ (autoDF (x := (x, y)) (y := y)) 0 (p +++ q) q 0. *)
+(* Proof. *)
+(*   apply has_cost_proj2. *)
+(* Qed. *)
+
+(* #[global] *)
+(* Instance has_cost_pair {A B C : AA} {x : A} {y : B} {z : C} {p q r} *)
+(*     (f : DF x y) (g : DF x z) *)
+(*   : has_cost_ f 0 p q 0 -> *)
+(*     has_cost_ g 0 p r 0 -> *)
+(*     has_cost_ (DF.pair f g) 0 p (q +++ r) 0. *)
+(* Proof. *)
+(* Admitted. *)
+
+(* #[global] *)
+(* Instance has_cost_autoDF_pair {A B C : AA} {x : A} {y : B} {z : C} {p q r} *)
+(*     `{!AutoDF x y, !AutoDF x z} *)
+(*   : has_cost_ (autoDF (x := x) (y := y)) 0 p q 0 -> *)
+(*     has_cost_ (autoDF (x := x) (y := z)) 0 p r 0 -> *)
+(*     has_cost_ (autoDF (x := x) (y := (y, z))) 0 p (q +++ r) 0. *)
+(* Proof. *)
+(*   apply has_cost_pair. *)
+(* Qed. *)
+
+(* Lemma var_cost {G A : AA} {g : G} {x : A} `{!AutoDF g x} {pre post} *)
+(*     {Hauto : has_cost_ (autoDF (x := g) (y := x)) 0 pre post 0} *)
+(*   : has_cost_ (var (g := g) x) 0 pre post 0. *)
+(* Proof. *)
+(*   exact Hauto. *)
+(* Qed. *)
+
+(* Lemma weaken_cost {G A : AA} (g : G) (x : A) (f : DF g x) m pre post n *)
+(*   : m <= n -> *)
+(*     has_cost_ f 0 pre post 0 -> *)
+(*     has_cost_ f m pre post n. *)
+(* Proof. *)
+(* Admitted. *)
+
+(* Lemma call_cost {G1 G2 A : AA} {g1 : G1} {g2 : G2} {x : A} `{!AutoDF g2 g1} *)
+(*     {f : DF g1 x} {pre1 pre2 post n m} *)
+(*     {Hauto : has_cost_ (autoDF (x := g2) (y := g1)) 0 pre2 pre1 0} *)
+(*   : has_cost_ f n pre1 post m -> *)
+(*     has_cost_ (call (g1 := g1) (g2 := g2) f) n pre2 post m. *)
+(* Proof. *)
+(*   unfold call. *)
+(*   intros H. eapply has_cost_compose. *)
+(*   - eapply weaken_cost; [ reflexivity | ]. *)
+(*     exact Hauto. *)
+(*   - apply H. *)
+(* Qed. *)
+
+(* Lemma if_cost {G A : AA} {g : G} {b : bool} {P : bool -> A} *)
+(*     (CASE : DF g b) *)
+(*     (TRUE : DF g (P true)) *)
+(*     (FALSE : DF g (P false)) *)
+(*     m n p q *)
+(*   : has_cost_ CASE 0 p zero 0 -> *)
+(*     (b = true -> has_cost_ TRUE m p q n) -> *)
+(*     (b = false -> has_cost_ FALSE m p q n) -> *)
+(*     has_cost_ (DF.if_ CASE TRUE FALSE) m p q n. *)
+(* Proof. *)
+(* Admitted. *)
+
+(* Theorem insTree_cost (t : Tree) (ts : list Tree) *)
+(*   : valid_Tree t -> *)
+(*     valid_Trees (rank t) ts -> *)
+(*     has_cost_ (insTreeDF t ts) (pot_trees ts) (zero +++ zero) zero (pot_trees (insTree t ts)). *)
+(* Proof. *)
+(* Admitted. (* *)
+(*   revert t; induction ts as [ | u ts IH]; intros t Vt Vts. *)
+(*   - cbn [insTreeDF]. *)
+(*     apply tick_cost. *)
+(*     apply match_list_nil_cost. *)
+(*     apply consD_cost. *)
+(*     + split; [ | split]; [ assumption | lia | exact I]. *)
+(*     + admit. *)
+(*     + apply var_cost. *)
+(*     + eapply weaken_cost. { unfold insert_budget; lia. } *)
+(*       apply nilD_cost. *)
+(*   - cbn [insTreeDF]. *)
+(*     apply tick_cost. *)
+(*     eapply match_list_cons_cost with (pot0 := pot_trees (rank t) (u :: ts)) (pot_tl := pot_trees (S (rank u)) ts) (m' := S (rank t)). *)
+(*     + apply weaken_cost. { reflexivity. } *)
+(*       apply var_cost. *)
+(*     + apply pot_trees_uncons. assumption. *)
+(*     + apply let_cost with (mid := zero) (m := S (rank t) + (rank u - rank t)). *)
+(*       { apply call_cost. admit. } *)
+(*       apply let_cost with (mid := zero) (m := S (rank t) + (rank u - rank t)). *)
+(*       { apply call_cost. admit. } *)
+(*       apply let_cost with (mid := zero) (m := S (rank t) + (rank u - rank t)). *)
+(*       { apply call_cost. admit. } *)
+(*       refine (if_cost _ _ _ _ _ _ _ _ _ _). *)
+(*       * intros Htrue. *)
+(*         cbn [insTree]. rewrite Htrue. *)
+(*         assert (Vts' : valid_Trees (S (rank t)) (u :: ts)). *)
+(*         { admit. } *)
+(*         assert (Vtts' : valid_Trees 0 (t :: u :: ts)). *)
+(*         { admit. } *)
+(*         apply consD_cost. *)
+(*         { assumption. } *)
+(*         { admit. } *)
+(*         { exact _.  } *)
+(*         { apply consD_cost. *)
+(*           { assumption. } *)
+(*           { lia. } *)
+(*           { exact _. } *)
+(*           { eapply weaken_cost. cbn. lia. apply var_cost. } } *)
+(*       * intros Hfalse. *)
+(*         apply let_cost with (mid := zero) (m := 1 + (rank u - r)). *)
+(*         { apply call_cost. admit. } *)
+(*         apply call_cost. *)
+(*         eapply weaken_cost. *)
+(* Qed. *)
+(* *) *)
+
+(* Lemma nodeD_cost_zero {r : AA} {s : r} {n x : nat} {ts : list Tree} *)
+(*     {pre : approx r -> nat} *)
+(*     `{!Subadditive pre} *)
+(*     (nD : DF s n) (xD : DF s x) (tsD : DF s ts) *)
+(*   : has_cost_ nD 0 pre zero 0 -> *)
+(*     has_cost_ xD 0 pre zero 0 -> *)
+(*     has_cost_ tsD 0 pre zero 0 -> *)
+(*     has_cost_ (nodeD nD xD tsD) 0 pre zero 0. *)
+(* Proof. *)
+(* Admitted. *)
+
+(* Theorem insert_cost (x : A) (h : Heap) *)
+(*   : valid_Heap h -> *)
+(*     has_cost_ (insertDF x h) 0 (zero +++ zero) zero insert_budget. *)
+(* Proof. (* *)
+(*   intros Vh. *)
+(*   change insert_budget with (0 + insert_budget). *)
+(*   apply let_cost with (mid := zero) (m := 0); [ admit | |]. *)
+(*   { apply nodeD_cost_zero. *)
+(*     + admit. *)
+(*     + admit. *)
+(*     + admit. } *)
+(*   change insert_budget with (0 + insert_budget). *)
+(*   apply let_cost with (mid := zero) (m := 0); [ admit | |]. *)
+(*   { admit. } *)
+(*   assert (HH : has_cost_ (insTreeDF (Node 0 x []) (trees h)) 0 (zero +++ pot_list) pot_list insert_budget). *)
+(*   { apply insTree_cost. assumption. } *)
+(*   admit. *) *)
+(* Admitted. *)
+
+(* (* *)
+(* Below: TODO *)
+(* *) *)
+
+(* Canonical AA_comparison : ApproxAlgebra := exact_AA comparison. *)
+
+(* Definition DF_compare {G A : ApproxAlgebra} {g : G} {b : comparison} {P : comparison -> A} *)
+(*   : DF g b -> DF g (P Lt) -> DF g (P Eq) -> DF g (P Gt) -> DF g (P b) := *)
+(*   (* TODO: use first argument *) *)
+(*   match b with *)
+(*   | Lt => fun _ p _ _ => p *)
+(*   | Eq => fun _ _ p _ => p *)
+(*   | Gt => fun _ _ _ p => p *)
+(*   end. *)
+
+(* Parameter compare_ : forall x y : nat, DF (x, y) (Nat.compare x y). *)
+
+(* Fixpoint mergeAuxDF (trs1 trs2 : list Tree) : DF (trs1, trs2) (mergeAux trs1 trs2) := *)
+(*   match_list (P := fun trs1 => mergeAux trs1 trs2) (var trs1) *)
+(*     (var trs2) *)
+(*     (fun t1 trs1' => *)
+(*       let trs1_ := t1 :: trs1' in *)
+(*       let fix merge_trs1DF trsR : DF (t1 :: trs1', t1, trs1', trsR) (mergeAux trs1_ trsR) := *)
+(*         match_list (P := fun trsR => mergeAux trs1_ trsR) (var trsR) *)
+(*         (var trs1_) *)
+(*         (fun t2 trs2' => *)
+(*           let trsR_ := t2 :: trs2' in *)
+(*           DF.let_ (call (rankDF t1)) *)
+(*           (DF.let_ (call (rankDF t2))  *)
+(*           (DF.let_ (call (compare_ (rank t1) (rank t2))) *)
+(*           (DF_compare (P := fun b => match b with Eq => _ | Lt => _ | Gt => _ end) *)
+(*              (var (Nat.compare (rank t1) (rank t2))) *)
+(*              (DF.let_ (call (mergeAuxDF trs1' trsR_)) *)
+(*               (consD (var t1) (call (mergeAuxDF trs1' trsR_)))) *)
+(*               (DF.let_ (call (linkDF t1 t2)) *)
+(*                 (DF.let_ (call (mergeAuxDF trs1' trs2')) *)
+(*                 (DF.let_ (call (insTreeDF (link t1 t2) (mergeAux trs1' trs2'))) *)
+(*                 (call (insTreeDF (link t1 t2) (mergeAux trs1' trs2')))))) *)
+(*               (consD (var t2) (call (merge_trs1DF trs2'))))))) *)
+(*       in *)
+(*       call (merge_trs1DF trs2)). *)
+
+(* Definition mergeDF (hp1 hp2 : Heap) : DF (hp1, hp2) (merge hp1 hp2) := *)
+(*   DF.let_ (treesD (var hp1))  *)
+(*   (DF.let_ (treesD (var hp2)) *)
+(*   (MkHeapD (call (mergeAuxDF _ _)))). *)
+
+(* Fixpoint removeMinAux (ts : list Tree) : option (Tree * list Tree) :=  *)
+(*   match ts with *)
+(*   | [] => None *)
+(*   | t :: ts' => match removeMinAux ts' with *)
+(*     | None => Some (t, []) *)
+(*     | Some (t', ts'') => if leb (root t) (root t') *)
+(*       then Some (t, ts') *)
+(*       else Some (t', t :: ts'') *)
+(*     end *)
+(*   end. *)
+
+(* Canonical AA_optionA (a : AA) : AA := *)
+(*   {| carrier := option a *)
+(*   ;  approx := T (option (approx a)) *)
+(*   ; AA_IsAA := TODO *)
+(*   ; AA_IsAS := TODO *)
+(*   ; AA_Setoid := TODO *)
+(*   |}. *)
+
+(* Definition noneD {G a : AA} {g : G} : DF g (None (A := a)). *)
+(* Admitted. *)
+
+(* Definition someD {G A : AA} {g : G} {x : A} *)
+(*   : DF g x -> DF g (Some x). *)
+(* Admitted. *)
+
+(* (* Auxiliary definition for match_option *) *)
+(* Definition force_some {G A : AA} {g : G} {x : A} *)
+(*   : DF (g, (Some x)) (g, x). *)
+(* Admitted. *)
+
+(* Definition match_option {G A B : AA} {P : option A -> B} {g : G} {xO : option A} *)
+(*     (CASE : DF g xO) *)
+(*     (NONE : DF g (P None)) *)
+(*     (SOME : forall x, DF (g, x) (P (Some x))) *)
+(*   : DF g (P xO) := *)
+(*   DF.bind CASE *)
+(*   match xO with *)
+(*   | None => DF.proj1 >>> NONE *)
+(*   | Some x => force_some >>> SOME x *)
+(*   end. *)
+
+(* Fixpoint removeMinAuxDF (ts : list Tree) : DF ts (removeMinAux ts). *)
+(* Admitted. (* match_list (P := fun ts => removeMinAux ts) (var ts) *)
+(*   noneD *)
+(*   (fun t ts' =>  *)
+(*     DF.let_ (call (removeMinAuxDF ts')) *)
+(*     (match_option (P  *)
+(*       (someD (DF.pair (var t) nilD)) *)
+(*       (fun p =>  *)
+(*         DF.let_ (call (rootDF t)) *)
+(*         (DF.let_ (DF.proj1 >>> call (rootDF _)) *)
+(*         (DF.let_ (DF.proj1 >>> call (lt_ (root _) (root t))) *)
+(*           (DF.if_ (P := fun b => if b then _ else _) *)
+(*             (DF.proj1 >>> var (root _ <? root t)) *)
+(*             (someD (DF.pair (DF.proj1) (DF.proj2 >>> consD (var t) _))) *)
+(*             (someD (DF.pair (var t) (var ts'))))))) *)
+(*     )).*) *)
+
+(* Definition heapConvert (p : Tree * (list Tree)) : (Tree * Heap) := *)
+(*   match p with *)
+(*   | (t, ts) => (t, MkHeap ts) *)
+(*   end. *)
+
+(* Definition heapConvertDF (p : Tree * (list Tree)) : DF p (heapConvert p). *)
+(* Admitted. *)
+
+(* Definition removeMinTree (hp : Heap)  *)
+(*   : option ((Tree) * (Heap)) := *)
+(*   match removeMinAux (trees hp) with *)
+(*   | Some (t, ts) => Some (t, MkHeap ts) *)
+(*   | None => None *)
+(*   end. *)
+
+(* (*Definition mergeDF (hp1 hp2 : Heap) : DF (hp1, hp2) (merge hp1 hp2) := *)
+(*   DF.let_ (treesD (var hp1))  *)
+(*   (DF.let_ (treesD (var hp2)) *)
+(*   (MkHeapD (call (mergeAuxDF _ _)))).*) *)
+
+(* (*Definition bind `{x : a, y : b, z : c} `(f : DF x y) `(g : DF (x, y) z) : DF x z := *)
+(*   pair (id x) f >>> g.*) *)
+
+(* (*Definition treesD {G : AA} {g : G} {h : Heap} (f : DF g h) : DF g (trees h).*) *)
+
+(* (*Definition match_option {G A B : AA} {P : option A -> B} {g : G} {xO : option A} *)
+(*     (CASE : DF g xO) *)
+(*     (NONE : DF g (P None)) *)
+(*     (SOME : forall x, DF (g, x) (P (Some x))) *)
+(*   : DF g (P xO) :=*) *)
+
+(* (* *)
+(* Definition var {G A : AA} {g : G} (x : A) `{AutoDF _ _ g x} : DF g x := autoDF. *)
+(* Definition call {x : A} `{AutoDF _ _ g2 g1} (f : DF g1 x) *)
+(*   : DF g2 x := autoDF >>> f.*) *)
+
+
+(* (*Fixpoint removeMinAuxDF (ts : list Tree) : DF ts (removeMinAux ts). *)
+
+(* Definition someD {G A : AA} {g : G} {x : A} *)
+(*   : DF g x -> DF g (Some x).*) *)
+
+(* Definition removeMinTreeDF (hp : Heap) : DF hp (removeMinTree hp). *)
+(* Admitted. *)
+(*   (*DF.let_  *)
+(*   (treesD (var hp)) *)
+
+(*   (*(g: DF (hp, trees hp) (removeMinTree hp))*) *)
+
+(*   (DF.let_ *)
+(*     (*(f : DF (hp, trees hp) (removeMinAux ts))*) (call (removeMinAuxDF _)) *)
+(*     (*(g : DF ((hp, trees hp), (removeMinAux ts)) (removeMinTree hp))*) *)
+(*     (match_option {P := fun h => removeMinAux h} *)
+(*       (*(CASE : DF ((hp, trees hp), (removeMinAux ts)) (removeMinAux ts))*) *)
+(*       (var (removeMinAux (trees hp))) *)
+(*       (*(NONE: DF ((hp, trees hp), (removeMinAux ts)) (P None))*) *)
+(*       noneD *)
+(*       (*(SOME: forall x, DF (((hp, trees hp), (removeMinAux ts)), x) (P (Some x))))*) *)
+(*       (fun p => someD (call (heapConvertDF p))) *)
+(*     )).*) *)
+(* (*  (DF.let_ (call (removeMinAuxDF _)) *)
+(*   (match_option (var (removeMinAux ts))  *)
+(*   noneD *)
+(*   (fun p => someD (DF.pair (DF.proj1) (DF.proj2 >>> MkHeapD _)))).*) *)
+
+(* Definition findMin (hp : Heap) *)
+(*   : option A := *)
+(*   match removeMinTree hp with *)
+(*   | None => None *)
+(*   | Some (t, _) => Some (root t) *)
+(*   end. *)
+
+(* Definition findMinDF (hp : Heap) : DF hp (findMin hp). *)
+(* Admitted. (* := *)
+(*   DF.let_ (call (removeMinTreeDF hp)) *)
+(*   (match_option (var _) *)
+(*     noneD *)
+(*     (fun p => DF.proj1 >>>  *)
+(*       DF.let_ (rootDF _) *)
+(*       (someD _))).*) *)
+
+(* Definition deleteMin (hp : Heap) *)
+(*   : Heap := *)
+(*   match removeMinTree hp with *)
+(*   | None => MkHeap [] *)
+(*   | Some (Node r v c, ts) => *)
+(*     merge (MkHeap (rev c)) ts *)
+(*   end. *)
+
+(* Definition revDF {A : AA} (xs : list A) : DF xs (rev xs). *)
+(* Admitted. *)
+
+(* Definition deleteMinDF (hp : Heap) : DF hp (deleteMin hp). *)
+(* Admitted. *)
+(* (*removeMinTreeDF hp >>> *)
+(*   (match_option (var _) *)
+(*   (MkHeapD nilD) *)
+(*   (fun p => DF.proj1 >>> *)
+(*     match_Tree *)
+(*     _ *)
+(*     (fun r1 v1 c1 =>  *)
+(*       DF.let_ (revD c1) (DF.let_ (MkHeapD _) (mergeDF _ (DF.proj2)))))).*) *)
+
+
+(* (* *)
+(* Canonical AABComparison : AA := *)
+(*   {| carrier := comparison |}. *)
+
+(* Definition if_ {a b : AA} {x : a} {cond : bool} *)
+(*   {f : bool -> b} *)
+(*   (i : DF x cond) *)
+(*   (thn : DF x (f true)) *)
+(*   (els : DF x (f false)) *)
+(*   : DF x (f cond). *)
+(* Proof. refine TODO. Defined.   *)
+
+(* (* Encoding of [Nat.compare] *) *)
+(* Definition natCompare {a b : AA} {c : a} {x y : nat}  *)
+(*   {f : comparison -> b} *)
+(*   (nats : DF c (x, y)) *)
+(*   (Lt_ : DF c (f Lt)) *)
+(*   (Eq_ : DF c (f Eq)) *)
+(*   (Gt_ : DF c (f Gt)) *)
+(*   : DF c (f (Nat.compare x y)). *)
+(* Proof. refine TODO. Defined. *)
+
+(* Fixpoint mergeAuxDF (trs1 trs2 : list Tree) : DF (trs1, trs2) (mergeAux trs1 trs2). *)
+(* Proof. *)
+(*   refine ((TODO : DF (trs1, trs2) (trs2, trs1)) >>> *)
+(*     (match_list (f := fun trs => mergeAux trs trs2) *)
+(*     _ (fun t1 trs1' => _))). *)
+(*   - cbn. refine TODO. *)
+(*   - refine ((TODO: DF (trs2, t1, trs1') (t1, trs1', trs2)) >>> *)
+(*     match_list (f := fun trs => mergeAux _ trs) *)
+(*     _ (fun t2 trs2' => _)). *)
+(*     + cbn [mergeAux]. refine (consD TODO TODO). *)
+(*     + cbn [mergeAux]. refine (natCompare  *)
+(*       (f := fun c => match c with *)
+(*         | Lt => _ *)
+(*         | Eq => _ *)
+(*         | Gt => _ *)
+(*         end) *)
+(*         _ *)
+(*         _ *)
+(*         _  *)
+(*         _). *)
+(*         * refine TODO. *)
+(*         * refine TODO. *)
+(*         * refine TODO. *)
+(*         * refine TODO.  *)
+(* Defined. *)
+
+(* Definition merge (hp1 hp2 : Heap) : Heap := *)
+(*   MkHeap (mergeAux (trees hp1) (trees hp2)). *)
+
+(* Definition mergeDF {hp1 hp2} : DF (hp1, hp2) (merge hp1 hp2). *)
+(* Proof. *)
+(*   refine (letDF (TODO >>> @treesD hp1) _). *)
+(*   refine (letDF (TODO >>> @treesD hp2) _). *)
+(*   refine (letDF (TODO >>> mergeAuxDF (trees hp1) (trees hp2)) _). *)
+(*   refine (proj2DF >>> MkHeapD _). *)
+(* Defined. *)
+
+(* Fixpoint removeMinAux (ts : list Tree) :=  *)
+(*   match ts with *)
+(*   | [] => None *)
+(*   | t :: ts' => match removeMinAux ts' with *)
+(*     | None => Some (t, []) *)
+(*     | Some (t', ts'') => if leb (root t) (root t') *)
+(*       then Some (t, ts') *)
+(*       else Some (t', t :: ts'') *)
+(*     end *)
+(*   end. *)
+
+(* Canonical AAoption (a : AA) : AA := *)
+(*   {| carrier := option a |}. *)
+
+(* (* Encoding of match on options *) *)
+(* Definition match_option {a b c : AA} {g : b} {f : option a -> c} {xM : option a} *)
+(*     (NONE : DF g (f None)) *)
+(*     (SOME : forall x, DF (g, x) (f (Some x))) *)
+(*   : DF (g, xM) (f xM) := *)
+(*   match xM with *)
+(*   | None => TODO >>> NONE *)
+(*   | Some x => TODO >>> (SOME x) *)
+(*   end. *)
+
+(* (* Encoding of None *) *)
+(* Definition noneD {a b : AA} {x : a} : DF x (None (A := b)). *)
+(* Proof. refine TODO. Defined. *)
+
+(* (* Encoding of (Some _) *) *)
+(* Definition someD {r a : AA} {s : r} {x : a} {xM : option a} (sD : DF s x) *)
+(*   : DF s (Some x). *)
+(* Proof. refine TODO. Defined. *)
+
+(* Fixpoint removeMinAuxDF {ts} : DF ts (removeMinAux ts). *)
+(* Proof. *)
+(*   refine (TODO >>>  *)
+(*     match_list (f := fun ts => removeMinAux ts) (g := ts) _ (fun t ts' => _)). (*TODO*) *)
+(*   - cbn. refine TODO. *)
+(*   - cbn. refine TODO. *)
+(* Defined. *)
+
+(* Definition removeMinTree (hp : Heap)  *)
+(*   : option ((Tree) * (Heap)) := *)
+(*   match removeMinAux (trees hp) with *)
+(*   | Some (t, ts) => Some (t, MkHeap ts) *)
+(*   | None => None *)
+(*   end. *)
+
+(* Definition removeMinTreeDF {hp} : DF hp (removeMinTree hp). *)
+(* Proof. *)
+(*   refine (letDF (TODO >>> @treesD hp) _). *)
+(*   refine (letDF (TODO >>> removeMinAuxDF) _). *)
+(*   refine (TODO >>> match_option  *)
+(*     (f := fun pM => match pM with *)
+(*       | None => None *)
+(*       | Some (t, ts) => Some (t, MkHeap ts)  *)
+(*       end) *)
+(*     (g := hp) (*TODO*) *)
+(*     (xM := removeMinAux (trees hp)) *)
+(*     _ (fun x => _)).  *)
+(*   - refine noneD. *)
+(*   - refine TODO. Unshelve. cbn. apply trees. assumption. (*TODO*) *)
+(* Defined. *)
+
+(* Definition findMin (hp : Heap) *)
+(*   : option A := *)
+(*   match removeMinTree hp with *)
+(*   | None => None *)
+(*   | Some (t, _) => Some (root t) *)
+(*   end. *)
+
+(* Definition findMindDF {hp} : DF hp (findMin hp). *)
+(* Proof. *)
+(*   refine (TODO >>> match_option  *)
+(*     (f := fun pM => match pM with *)
+(*       | None => None *)
+(*       | Some (t, _) => Some (root t)  *)
+(*   end) *)
+(*   (g := hp) (*TODO*) *)
+(*   (xM := removeMinTree hp) *)
+(*   _ (fun x => _)).  *)
+(*   - refine noneD. *)
+(*   - refine TODO. (*TODO*) *)
+(* Defined. *)
+
+(* Definition deleteMin (hp : Heap) *)
+(*   : Heap := *)
+(*   match removeMinTree hp with *)
+(*   | None => MkHeap [] *)
+(*   | Some (Node r v c, ts) => *)
+(*     merge (MkHeap (rev c)) ts *)
+(*   end. *)
+
+(* Definition deleteMinDF {hp} : DF hp (deleteMin hp). *)
+(* Proof. *)
+(*   refine (TODO >>> match_option  *)
+(*     (f := fun pM => match pM with *)
+(*       | None => MkHeap [] *)
+(*       | Some (Node r v c, ts) => *)
+(*         merge (MkHeap (rev c)) ts *)
+(*     end) *)
+(*   (g := hp) (*TODO*) *)
+(*   (xM := removeMinTree hp) *)
+(*   _ (fun x => _)).  *)
+(*   - refine TODO. *)
+(*   - refine TODO. (*TODO*) *)
+(* Defined.*) *)
+(* *) *)
+>>>>>>> 414ef5e (Work on binomial heap functional correctness)
